Adapting the code up to BasicMetaTheory. The BasicMetaTheory code only talks about the typing of the source theory currently (i.e. PType and Type are both used, as opposed to in the target theory).
Likely requires cleaning up and polishing in the future.

theories/autosubst/AST.sig
@@ -1,12 +1,3 @@
-list : Functor
-option : Functor
-
--- Global references
-gref : Type
-
--- Assumption references
-aref : Type
-
 -- Universe levels
 level : Type
 
@@ -14,11 +5,9 @@ level : Type
 
 term(var) : Type
 
-Sort : level -> term
+Typ : level -> term
+PTyp : level -> term
 
 Pi : term -> (bind term in term) -> term
 lam : term -> (bind term in term) -> term
 app : term -> term -> term
-
-const : gref -> "list" ("option" (term)) -> term
-assm : aref -> term
