theories/BasicMetaTheory.v
@@ -13,403 +13,179 @@ Import CombineNotations.
 
 Set Default Goal Selector "!".
 
-(** Better induction principle for [term] *)
-
-Lemma term_rect :
-   ∀ (P : term → Type),
-    (∀ n, P (var n)) →
-    (∀ i, P (Sort i)) →
-    (∀ A, P A → ∀ B, P B → P (Pi A B)) →
-    (∀ A, P A → ∀ t, P t → P (lam A t)) →
-    (∀ u, P u → ∀ v, P v → P (app u v)) →
-    (∀ (c : gref) (ξ : instance), All (onSomeT P) ξ → P (const c ξ)) →
-    (∀ (x : aref), P (assm x)) →
-    ∀ t, P t.
-Proof.
-  intros P hvar hsort hpi hlam happ hconst hassm.
-  fix aux 1. move aux at top.
-  intro t. destruct t.
-  6:{
-    eapply hconst.
-    revert l. fix aux1 1.
-    intro ξ. destruct ξ as [| t ξ]. 1: constructor.
-    constructor. 2: eauto.
-    destruct t. 2: constructor.
-    cbn. auto.
-  }
-  all: match goal with h : _ |- _ => eapply h end.
-  all: eauto.
-Defined.
-
-(** Better induction principle for [gscope] *)
-
-Lemma gscope_ind :
-  ∀ Σ (P : term → Prop),
-  (∀ x, P (var x)) →
-  (∀ i, P (Sort i)) →
-  (∀ A B, gscope Σ A → P A → gscope Σ B → P B → P (Pi A B)) →
-  (∀ A t, gscope Σ A → P A → gscope Σ t → P t → P (lam A t)) →
-  (∀ u v, gscope Σ u → P u → gscope Σ v → P v → P (app u v)) →
-  (∀ c ξ Ξ' A t,
-    Σ c = Some (Def Ξ' A t) →
-    gscope_instance Σ ξ →
-    Forall (OnSome P) ξ →
-    P (const c ξ)
-  ) →
-  (∀ x, P (assm x)) →
-  ∀ t, gscope Σ t → P t.
-Proof.
-  intros Σ P hvar hsort hpi hlam happ hconst hassm.
-  fix aux 2. move aux at top.
-  intros t h. destruct h as [| | | | | c ξ ??? hc h |].
-  6:{
-    eapply hconst. 1,2: eassumption.
-    revert ξ h.
-    fix aux1 2.
-    intros ξ h. destruct h as [| u ξ hu hξ].
-    - constructor.
-    - constructor. 2: eauto.
-      destruct hu.
-      + constructor.
-      + constructor. eauto.
-  }
-  all: match goal with h : _ |- _ => solve [ eapply h ; eauto ] end.
-Qed.
-
-(** Better induction principle for [conversion] *)
-
-Lemma conversion_ind :
-  ∀ (Σ : gctx) Ξ (P : term → term → Prop),
-    (∀ A t u, P (app (lam A t) u) (t <[ u.. ])) →
-    (∀ c ξ Ξ' A t,
-      Σ c = Some (Def Ξ' A t) →
-      inst_equations Σ Ξ ξ Ξ' →
-      inst_equations_ P ξ Ξ' →
-      closed t = true →
-      P (const c ξ) (inst ξ t)
-    ) →
-    (∀ n rl σ,
-      ictx_get Ξ n = Some (Comp rl) →
-      let Θ := rl.(cr_env) in
-      let k := length Θ in
-      let lhs := rl.(cr_pat) in
-      let rhs := rl.(cr_rep) in
-      scoped k lhs = true →
-      scoped k rhs = true →
-      P (lhs <[ σ ]) (rhs <[ σ ])
-    ) →
-    (∀ A A' B B',
-      Σ ;; Ξ ⊢ A ≡ A' →
-      P A A' →
-      Σ ;; Ξ ⊢ B ≡ B' →
-      P B B' →
-      P (Pi A B) (Pi A' B')
-    ) →
-    (∀ A A' t t',
-      Σ ;; Ξ ⊢ A ≡ A' →
-      P A A' →
-      Σ ;; Ξ ⊢ t ≡ t' →
-      P t t' →
-      P (lam A t) (lam A' t')
-    ) →
-    (∀ u u' v v',
-      Σ ;; Ξ ⊢ u ≡ u' →
-      P u u' →
-      Σ ;; Ξ ⊢ v ≡ v' →
-      P v v' →
-      P (app u v) (app u' v')
-    ) →
-    (∀ c ξ ξ',
-      Forall2 (option_rel (conversion Σ Ξ)) ξ ξ' →
-      Forall2 (option_rel P) ξ ξ' →
-      P (const c ξ) (const c ξ')
-    ) →
-    (∀ u, P u u) →
-    (∀ u v, Σ ;; Ξ ⊢ u ≡ v → P u v → P v u) →
-    (∀ u v w,
-      Σ ;; Ξ ⊢ u ≡ v →
-      P u v →
-      Σ ;; Ξ ⊢ v ≡ w →
-      P v w →
-      P u w
-    ) →
-    ∀ u v, Σ ;; Ξ ⊢ u ≡ v → P u v.
-Proof.
-  intros Σ Ξ P hbeta hunfold hred hpi hlam happ hconst hrefl hsym htrans.
-  fix aux 3. move aux at top.
-  intros u v h. destruct h.
-  7:{
-    eapply hconst. 1: assumption.
-    revert ξ ξ' H.
-    fix aux1 3.
-    intros ξ ξ' h. destruct h as [| u u' ξ ξ' hu hξ].
-    - constructor.
-    - constructor. 2: eauto.
-      destruct hu. 1: constructor.
-      constructor. eauto.
-  }
-  2:{
-    eapply hunfold. 1,2,4: eassumption.
-    intros x rl hx. specialize (H0 _ _ hx) as (? & ? & ?).
-    intuition eauto.
-  }
-  all: match goal with h : _ |- _ => solve [ eapply h ; eauto ] end.
-Qed.
-
 (** Better induction principle for [typing] *)
 
-Lemma typing_ind :
-  ∀ Σ Ξ (P : ctx → term → term → Prop),
+Check styping_ind.
+
+Lemma styping_ind :
+  ∀ (P : ctx → term → term → Prop),
     (∀ Γ x A, nth_error Γ x = Some A → P Γ (var x) (Nat.add (S x) ⋅ A)) →
-    (∀ Γ i, P Γ (Sort i) (Sort (S i))) →
+    (∀ Γ i, P Γ (Typ i) (Typ (S i))) →
+    (∀ Γ i, P Γ (PTyp i) (PTyp (S i))) →
+
     (∀ Γ i j A B,
-      Σ ;; Ξ | Γ ⊢ A : Sort i →
-      P Γ A (Sort i) →
-      Σ ;; Ξ | Γ,, A ⊢ B : Sort j →
-      P (Γ,, A) B (Sort j) →
-      P Γ (Pi A B) (Sort (Nat.max i j))
+      Γ ⊢ A : Typ i → P Γ A (Typ i) →
+      Γ,, A ⊢ B : Typ j → P (Γ,, A) B (Typ j) →
+      P Γ (Pi A B) (Typ (Nat.max i j))
+    ) →
+    (∀ Γ i j A B,
+      Γ ⊢ A : PTyp i → P Γ A (PTyp i) →
+      Γ,, A ⊢ B : PTyp j → P (Γ,, A) B (PTyp j) →
+      P Γ (Pi A B) (PTyp (Nat.max i j))
+    ) →
+    (∀ Γ i j A B,
+      Γ ⊢ A : PTyp i → P Γ A (PTyp i) →
+      Γ,, A ⊢ B : Typ j → P (Γ,, A) B (Typ j) →
+      P Γ (Pi A B) (Typ (Nat.max i j))
+    ) →
+    (∀ Γ i j A B,
+      Γ ⊢ A : Typ i → P Γ A (Typ i) →
+      Γ,, A ⊢ B : PTyp j → P (Γ,, A) B (PTyp j) →
+      P Γ (Pi A B) (PTyp (Nat.max i j))
+    ) →
+    
+    (∀ Γ i j A B t,
+      Γ ⊢ A : Typ i → P Γ A (Typ i) →
+      Γ,, A ⊢ B : Typ j → P (Γ,, A) B (Typ j) →
+      Γ,, A ⊢ t : B → P (Γ,, A) t B →
+      P Γ (lam A t) (Pi A B)
     ) →
     (∀ Γ i j A B t,
-      Σ ;; Ξ | Γ ⊢ A : Sort i →
-      P Γ A (Sort i) →
-      Σ ;; Ξ | Γ,, A ⊢ B : Sort j →
-      P (Γ,, A) B (Sort j) →
-      Σ ;; Ξ | Γ,, A ⊢ t : B →
-      P (Γ,, A) t B → P Γ (lam A t) (Pi A B)
+      Γ ⊢ A : PTyp i → P Γ A (PTyp i) →
+      Γ,, A ⊢ B : PTyp j → P (Γ,, A) B (PTyp j) →
+      Γ,, A ⊢ t : B → P (Γ,, A) t B →
+      P Γ (lam A t) (Pi A B)
     ) →
+    (∀ Γ i j A B t,
+      Γ ⊢ A : PTyp i → P Γ A (PTyp i) →
+      Γ,, A ⊢ B : Typ j → P (Γ,, A) B (Typ j) →
+      Γ,, A ⊢ t : B → P (Γ,, A) t B → 
+      P Γ (lam A t) (Pi A B)
+    ) →
+    (∀ Γ i j A B t,
+      Γ ⊢ A : Typ i → P Γ A (Typ i) →
+      Γ,, A ⊢ B : PTyp j → P (Γ,, A) B (PTyp j) →
+      Γ,, A ⊢ t : B → P (Γ,, A) t B →
+      P Γ (lam A t) (Pi A B)
+    ) →
+    
     (∀ Γ i j A B t u,
-      Σ ;; Ξ | Γ ⊢ t : Pi A B →
-      P Γ t (Pi A B) →
-      Σ ;; Ξ | Γ ⊢ u : A →
-      P Γ u A → Σ ;; Ξ | Γ ⊢ A : Sort i →
-      P Γ A (Sort i) → Σ ;; Ξ | Γ,, A ⊢ B : Sort j →
-      P (Γ,, A) B (Sort j) →
+      Γ ⊢ t : Pi A B → P Γ t (Pi A B) →
+      Γ ⊢ u : A → P Γ u A →
+      Γ ⊢ A : Typ i → P Γ A (Typ i) →
+      Γ,, A ⊢ B : Typ j → P (Γ,, A) B (Typ j) →
       P Γ (app t u) (B <[ u..])
     ) →
-    (∀ Γ c ξ Ξ' A t,
-      Σ c = Some (Def Ξ' A t) →
-      inst_typing Σ Ξ Γ ξ Ξ' →
-      inst_typing_ (conversion Σ Ξ) (P Γ) ξ Ξ' →
-      closed A = true →
-      P Γ (const c ξ) (inst ξ A)
+    (∀ Γ i j A B t u,
+      Γ ⊢ t : Pi A B → P Γ t (Pi A B) →
+      Γ ⊢ u : A → P Γ u A →
+      Γ ⊢ A : PTyp i → P Γ A (PTyp i) →
+      Γ,, A ⊢ B : PTyp j → P (Γ,, A) B (PTyp j) →
+      P Γ (app t u) (B <[ u..])
     ) →
-    (∀ Γ x A,
-      ictx_get Ξ x = Some (Assm A) →
-      closed A = true →
-      P Γ (assm x) A
+    (∀ Γ i j A B t u,
+      Γ ⊢ t : Pi A B → P Γ t (Pi A B) →
+      Γ ⊢ u : A → P Γ u A →
+      Γ ⊢ A : PTyp i → P Γ A (PTyp i) →
+      Γ,, A ⊢ B : Typ j → P (Γ,, A) B (Typ j) →
+      P Γ (app t u) (B <[ u..])
     ) →
+    (∀ Γ i j A B t u,
+      Γ ⊢ t : Pi A B → P Γ t (Pi A B) →
+      Γ ⊢ u : A → P Γ u A →
+      Γ ⊢ A : Typ i → P Γ A (Typ i) →
+      Γ,, A ⊢ B : PTyp j → P (Γ,, A) B (PTyp j) →
+      P Γ (app t u) (B <[ u..])
+    ) →
+    
     (∀ Γ i A B t,
-      Σ ;; Ξ | Γ ⊢ t : A →
-      P Γ t A →
-      Σ ;; Ξ ⊢ A ≡ B →
-      Σ ;; Ξ | Γ ⊢ B : Sort i →
-      P Γ B (Sort i) →
+      Γ ⊢ t : A → P Γ t A → A ≡ B →
+      Γ ⊢ B : Typ i → P Γ B (Typ i) →
       P Γ t B
     ) →
-    ∀ Γ t A, Σ ;; Ξ | Γ ⊢ t : A → P Γ t A.
+    (∀ Γ i A B t,
+      Γ ⊢ t : A → P Γ t A → A ≡ B →
+      Γ ⊢ B : PTyp i → P Γ B (PTyp i) →
+      P Γ t B
+    ) →
+    
+    ∀ Γ t A, Γ ⊢ t : A → P Γ t A.
 Proof.
-  intros Σ Ξ P hvar hsort hpi hlam happ hconst hassm hconv.
+  intros P
+    hvar htyp hptyp
+    hpiT hpiP hpiPT hpiTP
+    hlamT hlamP hlamPT hlamTP
+    happT happP happPT happTP
+    hconvT hconvP.
   fix aux 4. move aux at top.
-  intros Γ t A h. destruct h as [| | | | | ????? hc h hA | |].
-  6:{
-    eapply hconst. 1,2,4: eassumption.
-    clear hc.
-    induction h in |- *; constructor; eauto.
-  }
-  all: match goal with h : _ |- _ => solve [ eapply h ; eauto ] end.
-Qed.
-
-
-Lemma inst_typing_nth_error_gen {conv typ ξ Ξ} n :
-  inst_typing_ conv typ ξ Ξ →
-  match nth_error (rev ξ) n, nth_error Ξ n with
-  | None, None => True
-  | Some (Some t), Some (Assm A) => closed A = true ∧ iscope (skipn (S n) Ξ) A ∧ typ t (inst (firstn (length ξ - S n) ξ) A)
-  | Some None, Some (Comp rl) =>
-    let m := length rl.(cr_env) in
-    (* let Θ := ctx_inst ξ rl.(cr_env) in *)
-    let lhs := inst (liftn m (firstn (length ξ - S n) ξ)) rl.(cr_pat) in
-    let rhs := inst (liftn m (firstn (length ξ - S n) ξ)) rl.(cr_rep) in
-    scoped m rl.(cr_pat) = true ∧
-    iscope (skipn (S n) Ξ) rl.(cr_pat) ∧
-    scoped m rl.(cr_rep) = true ∧
-    iscope (skipn (S n) Ξ) rl.(cr_rep) ∧
-    conv lhs rhs
-  | _, _ => False
-  end.
-Proof.
-  induction 1 in n.
-  1: now rewrite !nth_error_nil.
-  all: rewrite rev_app_distr; cbn.
-  all: destruct n; cbn.
-  2,4: rewrite length_app, Nat.add_comm, firstn_app; cbn;
-    replace (length ξ - S n - length ξ) with 0 by lia; cbn;
-    rewrite app_nil_r; eapply IHinst_typing_; eassumption.
-  all: rewrite length_app; cbn; rewrite Nat.add_sub, firstn_app, firstn_all, Nat.sub_diag; cbn; rewrite app_nil_r.
-  - repeat split; try assumption.
-  - repeat split; assumption.
-Qed.
-
-Lemma inst_typing_length {conv typ ξ Ξ} :
-  inst_typing_ conv typ ξ Ξ →
-  length ξ = length Ξ.
-Proof. induction 1; eauto. all: rewrite length_app, Nat.add_comm. all: now cbn; f_equal. Qed.
-
-
-Lemma inst_typing_nth_error_gen' {conv typ ξ Ξ} n :
-  inst_typing_ conv typ ξ Ξ →
-  match nth_error ξ n, ictx_get Ξ n with
-  | None, None => True
-  | Some (Some t), Some (Assm A) => closed A = true ∧ iscope (skipn (length Ξ - n) Ξ) A ∧ typ t (inst (firstn n ξ) A)
-  | Some None, Some (Comp rl) =>
-    let m := length rl.(cr_env) in
-    (* let Θ := ctx_inst ξ rl.(cr_env) in *)
-    let lhs := inst (liftn m (firstn n ξ)) rl.(cr_pat) in
-    let rhs := inst (liftn m (firstn n ξ)) rl.(cr_rep) in
-    scoped m rl.(cr_pat) = true ∧
-    iscope (skipn (length Ξ - n) Ξ) rl.(cr_pat) ∧
-    scoped m rl.(cr_rep) = true ∧
-    iscope (skipn (length Ξ - n) Ξ) rl.(cr_rep) ∧
-    conv lhs rhs
-  | _, _ => False
-  end.
-Proof.
-  intros H. unfold ictx_get.
-  apply inst_typing_length in H as hlen.
-  destruct (Nat.ltb_spec n (length ξ)).
-  - replace (firstn n ξ) with (firstn (length ξ - S (length ξ - S n)) ξ) by (f_equal; lia).
-    replace (skipn (Datatypes.length Ξ - n) Ξ) with (skipn (S (Datatypes.length ξ - S n)) Ξ) by (f_equal; lia).
-    replace (nth_error ξ n) with (nth_error (rev ξ) (length ξ - S n)).
-    1: replace (nth_error (rev Ξ) n) with (nth_error Ξ (length ξ - S n)).
-    1: now apply inst_typing_nth_error_gen with (n := length ξ - S n).
-    + rewrite hlen in H0. rewrite hlen.
-      rewrite nth_error_rev.
-      apply Nat.ltb_lt in H0 as ->. auto.
-    + rewrite nth_error_rev.
-      destruct (Nat.ltb_spec (length ξ - S n) (length ξ)).
-      * f_equal. lia.
-      * lia.
-  - apply nth_error_None in H0 as hnone. rewrite hnone.
-    rewrite hlen, <- length_rev in H0.
-    apply nth_error_None in H0 as hnone'. rewrite hnone'. auto.
-Qed.
-
-Lemma inst_typing_nth_error_assm conv typ ξ Ξ n t :
-  inst_typing_ conv typ ξ Ξ →
-  nth_error ξ n = Some (Some t) →
-  ∃ A, ictx_get Ξ n = Some (Assm A) ∧
-    closed A = true ∧
-    iscope (skipn (length Ξ - n) Ξ) A ∧
-    typ t (inst (firstn n ξ) A).
-Proof.
-  intro H.
-  pose proof (inst_typing_nth_error_gen' n H).
-  intros e; rewrite e in H0.
-  destruct (ictx_get Ξ n) as [[]|]; try easy.
-  exists A; split; auto.
-Qed.
-
-Lemma inst_typing_ictx_get_assm conv typ ξ Ξ n A :
-  inst_typing_ conv typ ξ Ξ →
-  ictx_get Ξ n = Some (Assm A) →
-  closed A = true ∧
-  iscope (skipn (length Ξ - n) Ξ) A ∧
-  ∃ t, nth_error ξ n = Some (Some t) ∧
-    typ t (inst (firstn n ξ) A).
-Proof.
-  intro H.
-  pose proof (inst_typing_nth_error_gen' n H).
-  intros e; rewrite e in H0.
-  destruct (nth_error ξ n) as [[]|]; try easy.
-  split; try apply H0.
-  split; try apply H0.
-  exists t; split; auto.
-  apply H0.
-Qed.
-
-Lemma inst_typing_nth_error_comp conv typ ξ Ξ n :
-  inst_typing_ conv typ ξ Ξ →
-  nth_error ξ n = Some None →
-  ∃ rl, ictx_get Ξ n = Some (Comp rl) ∧
-    let m := length rl.(cr_env) in
-    (* let Θ := ctx_inst ξ rl.(cr_env) in *)
-    let lhs := inst (liftn m (firstn n ξ)) rl.(cr_pat) in
-    let rhs := inst (liftn m (firstn n ξ)) rl.(cr_rep) in
-    scoped m rl.(cr_pat) = true ∧
-    iscope (skipn (Datatypes.length Ξ - n) Ξ) rl.(cr_pat) ∧
-    scoped m rl.(cr_rep) = true ∧
-    iscope (skipn (Datatypes.length Ξ - n) Ξ) rl.(cr_rep) ∧
-    conv lhs rhs.
-Proof.
-  intro H.
-  pose proof (inst_typing_nth_error_gen' n H).
-  intros e; rewrite e in H0.
-  destruct (ictx_get Ξ n) as [[]|]; try easy.
-  exists rl; split; auto.
-Qed.
-
-Lemma inst_typing_ictx_get_comp conv typ ξ Ξ n rl :
-  inst_typing_ conv typ ξ Ξ →
-  ictx_get Ξ n = Some (Comp rl) →
-  nth_error ξ n = Some None ∧
-  let m := length rl.(cr_env) in
-  (* let Θ := ctx_inst ξ rl.(cr_env) in *)
-  let lhs := inst (liftn m (firstn n ξ)) rl.(cr_pat) in
-  let rhs := inst (liftn m (firstn n ξ)) rl.(cr_rep) in
-  scoped m rl.(cr_pat) = true ∧
-  iscope (skipn (Datatypes.length Ξ - n) Ξ) rl.(cr_pat) ∧
-  scoped m rl.(cr_rep) = true ∧
-  iscope (skipn (Datatypes.length Ξ - n) Ξ) rl.(cr_rep) ∧
-  conv lhs rhs.
-Proof.
-  intro H.
-  pose proof (inst_typing_nth_error_gen' n H).
-  intros e; rewrite e in H0.
-  destruct (nth_error ξ n) as [[]|]; try easy.
-Qed.
-
-(** Reasoning principle on [inst_typing] *)
-
-Lemma inst_typing_prop_ih conv ξ Ξ' P :
-  inst_typing_ conv (λ t _, P t) ξ Ξ' →
-  Forall (OnSome P) ξ.
-Proof.
-  induction 1.
-  1: constructor.
-  all: apply Forall_app; split; auto.
-  all: repeat constructor.
-  assumption.
+  intros Γ t A h.
+  destruct h as [n| |
+                |????[h1|h2]
+                |????[h1|h2]
+                |?????[h1|h2][h1'|h2']
+                |????????[h1|h2][h1'|h2']
+                |??????[h1|h2]].
+  - now apply hvar.
+  - now apply htyp.
+  - now apply hptyp.
+  - apply hpiTP.
+    all: try apply aux; easy.
+  - apply hpiP.
+    all: try apply aux; easy.
+  - apply hpiT.
+    all: try apply aux; easy.
+  - apply hpiPT.
+    all: try apply aux; easy.
+  - apply (hlamT _ i j).
+    all: try apply aux; easy.
+  - apply (hlamTP _ i j).
+    all: try apply aux; easy.
+  - apply (hlamPT _ i j).
+    all: try apply aux; easy.
+  - apply (hlamP _ i j).
+    all: try apply aux; easy.
+  - apply (happT _ i j A).
+    all: try apply aux; easy.
+  - apply (happTP _ i j A).
+    all: try apply aux; easy.
+  - apply (happPT _ i j A).
+    all: try apply aux; easy.
+  - apply (happP _ i j A).
+    all: try apply aux; easy.
+  - apply (hconvT _ i A).
+    all: try apply aux; easy.
+  - apply (hconvP _ i A).
+    all: try apply aux; easy.
 Qed.
 
 (** Typing implies scoping *)
 
-Lemma typing_scoped Σ Ξ Γ t A :
-  Σ ;; Ξ | Γ ⊢ t : A →
+Check styping_ind.
+
+Lemma styping_scoped Γ t A :
+  Γ ⊢ t : A →
   scoped (length Γ) t = true.
 Proof.
   intro h.
-  induction h using typing_ind.
+  induction h using styping_ind.
   all: try solve [ cbn - ["<?"] in * ; eauto ].
   all: try solve [
     cbn - ["<?"] in * ;
     rewrite Bool.andb_true_iff in * ;
     intuition eauto
   ].
-  - cbn - ["<?"]. rewrite Nat.ltb_lt. eapply nth_error_Some. congruence.
-  - cbn. eapply forallb_forall. intros u hu.
-    eapply In_nth_error in hu as [n hn].
-    destruct u. 2: reflexivity.
-    cbn.
-    eapply inst_typing_nth_error_assm in hn as (A' & _ & _ & _ & hn); eauto.
-    cbn in hn. assumption.
-Qed.
+  simpl. rewrite Nat.ltb_lt, <-nth_error_Some.
+  congruence.
+Qed. 
 
-Lemma typing_closed Σ Ξ t A :
-  Σ ;; Ξ | ∙ ⊢ t : A →
+Lemma styping_closed t A :
+  ∙ ⊢ t : A →
   closed t = true.
+
 Proof.
   intros h.
-  eapply typing_scoped with (Γ := ∙).
+
+  eapply styping_scoped with (Γ := ∙).
   eassumption.
 Qed.
 
@@ -501,86 +277,11 @@ Proof.
   - apply extRen_term. intro. core.unfold_funcomp. lia.
 Qed.
 
-Lemma ren_instance_comp :
-  ∀ ρ ρ' ξ,
-    ren_instance ρ (ren_instance ρ' ξ) = ren_instance (ρ' >> ρ) ξ.
-Proof.
-  intros ρ ρ' ξ.
-  rewrite map_map.
-  apply map_ext. intro u.
-  rewrite option_map_option_map.
-  apply option_map_ext. intro t.
-  rasimpl. reflexivity.
-Qed.
-
-Lemma lift_ren_instance :
-  ∀ ρ ξ,
-    lift_instance (ren_instance ρ ξ) =
-    ren_instance (upRen_term_term ρ) (lift_instance ξ).
-Proof.
-  intros ρ ξ.
-  rewrite !ren_instance_comp. reflexivity.
-Qed.
-
-Lemma ren_instance_ext ρ ζ ξ :
-  (∀ n, ρ n = ζ n) →
-  ren_instance ρ ξ = ren_instance ζ ξ.
-Proof.
-  intros h.
-  apply map_ext. intro.
-  apply option_map_ext. intro.
-  apply extRen_term. assumption.
-Qed.
-
-Lemma liftn_liftn n m ξ :
-  liftn n (liftn m ξ) = liftn (n + m) ξ.
-Proof.
-  rewrite ren_instance_comp.
-  apply ren_instance_ext. unfold core.funcomp. intro. lia.
-Qed.
-
 Fixpoint uprens k (ρ : nat → nat) :=
   match k with
   | 0 => ρ
   | S k => upRen_term_term (uprens k ρ)
   end.
-
-Lemma liftn_ren_instance n ρ ξ :
-  liftn n (ren_instance ρ ξ) = ren_instance (uprens n ρ) (liftn n ξ).
-Proof.
-  rewrite 2!ren_instance_comp. apply ren_instance_ext.
-  intros m. unfold core.funcomp.
-  induction n as [| n ih] in m, ρ |- *.
-  - reflexivity.
-  - cbn. unfold core.funcomp. rewrite <- ih.
-    reflexivity.
-Qed.
-
-Lemma iget_ren ξ x ρ :
-  iget (ren_instance ρ ξ) x = ρ ⋅ (iget ξ x).
-Proof.
-  unfold iget.
-  rewrite nth_error_map.
-  destruct (nth_error ξ x) as [[] |]. all: reflexivity.
-Qed.
-
-Lemma ren_inst :
-  ∀ ρ ξ t,
-    ρ ⋅ (inst ξ t) = inst (ren_instance ρ ξ) (ρ ⋅ t).
-Proof.
-  intros ρ ξ t.
-  induction t using term_rect in ρ, ξ |- *.
-  all: try solve [ cbn ; rewrite ?lift_ren_instance ; f_equal ; eauto ].
-  - cbn. f_equal.
-    rewrite !map_map. apply map_ext_All.
-    eapply All_impl. 2: eassumption.
-    intros u h.
-    change @core.option_map with @option_map.
-    rewrite !option_map_option_map. apply option_map_ext_onSomeT.
-    eapply onSomeT_impl. 2: eassumption.
-    cbn. intros t ht. auto.
-  - cbn. rewrite iget_ren. reflexivity.
-Qed.
 
 Lemma scoped_ren :
   ∀ ρ k t,
@@ -605,18 +306,6 @@ Proof.
     + destruct k. 1: lia.
       cbn. core.unfold_funcomp. f_equal.
       apply ih. lia.
-  - cbn in *. f_equal.
-    rewrite <- map_id. apply map_ext_All.
-    apply forallb_All in h. move h at top.
-    eapply All_prod in h. 2: eassumption.
-    eapply All_impl. 2: eassumption. clear.
-    cbn. intros o [h1 h2].
-    change @core.option_map with @option_map.
-    apply option_map_id_onSomeT.
-    rewrite onSomeb_onSome in h2. eapply onSome_onSomeT in h2.
-    eapply onSomeT_prod in h1. 2: eassumption.
-    eapply onSomeT_impl. 2: eassumption. clear.
-    cbn. intros t [h1 h2]. eauto.
 Qed.
 
 Corollary closed_ren :
@@ -628,74 +317,16 @@ Proof.
   eapply scoped_ren in h. eauto.
 Qed.
 
-Lemma ren_instance_id ξ :
-  ren_instance id ξ = ξ .
-Proof.
-  rewrite <- map_id. apply map_ext. intro.
-  rewrite <- option_map_id. apply option_map_ext. intro.
-  rasimpl. reflexivity.
-Qed.
-
-Lemma ren_instance_id_ext ρ ξ :
-  (∀ n, ρ n = n) →
-  ren_instance ρ ξ = ξ.
-Proof.
-  intro h.
-  etransitivity. 2: eapply ren_instance_id.
-  apply ren_instance_ext. assumption.
-Qed.
-
-Corollary closed_ren_instance ρ ξ :
-  closed_instance ξ = true →
-  ren_instance ρ ξ = ξ.
-Proof.
-  intros h.
-  etransitivity. 2: apply ren_instance_id.
-  apply map_ext_All. eapply All_impl.
-  2:{ apply forallb_All. eassumption. }
-  cbn. intros o ho%onSomeb_onSome%onSome_onSomeT.
-  apply option_map_ext_onSomeT. eapply onSomeT_impl. 2: eassumption.
-  cbn. rasimpl. apply closed_ren.
-Qed.
-
-Lemma inst_equations_ren_ih Σ Ξ ρ ξ Ξ' :
-  inst_equations Σ Ξ ξ Ξ' →
-  inst_equations_ (λ u v, ∀ ρ, Σ ;; Ξ ⊢ ρ ⋅ u ≡ ρ ⋅ v) ξ Ξ' →
-  inst_equations Σ Ξ (ren_instance ρ ξ) Ξ'.
-Proof.
-  intros h ih.
-  intros x rl hx m. cbn.
-  rewrite nth_error_map.
-  rewrite liftn_ren_instance.
-  specialize (ih _ _ hx) as (e & hl & hr & ih).
-  fold m in hl, hr, ih.
-  specialize ih with (ρ := uprens m ρ).
-  rewrite e. cbn.
-  rewrite 2!ren_inst in ih.
-  rewrite 2!scoped_ren in ih. 2,3: eassumption.
-  intuition eauto.
-Qed.
-
-Lemma conv_ren Σ Ξ ρ u v :
-  Σ ;; Ξ ⊢ u ≡ v →
-  Σ ;; Ξ ⊢ ρ ⋅ u ≡ ρ ⋅ v.
+Lemma conv_ren ρ u v :
+  u ≡ v →
+  ρ ⋅ u ≡ ρ ⋅ v.
 Proof.
   intros h.
   induction h using conversion_ind in ρ |- *.
-  all: try solve [ rasimpl ; econstructor ; eauto ].
-  - rasimpl. eapply meta_conv_trans_r. 1: econstructor.
-    rasimpl. reflexivity.
-  - rasimpl. eapply conv_trans. 1: econstructor. 1,3: eassumption.
-    1: eauto using inst_equations_ren_ih.
-    rewrite ren_inst. rewrite closed_ren. 2: assumption.
-    ttconv.
-  - cbn. constructor.
-    rewrite Forall2_map_l, Forall2_map_r.
-    eapply Forall2_impl. 2: eassumption.
-    intros o o' h.
-    rewrite option_rel_map_l, option_rel_map_r.
-    eapply option_rel_impl. 2: eassumption.
-    cbn. intros u v ih. eauto.
+  all: try solve [ rasimpl ; econstructor ; eauto ].  
+  rasimpl. apply (conv_trans _ (((0 .: ρ >> S) ⋅ t) <[ (ρ ⋅ u)..])).
+  - constructor.
+  - rasimpl. constructor.
 Qed.
 
 Fixpoint ren_ctx ρ Γ {struct Γ} :=
@@ -744,102 +375,35 @@ Proof.
     rasimpl. reflexivity.
 Qed.
 
-Lemma length_ctx_inst ξ Γ :
-  length (ctx_inst ξ Γ) = length Γ.
-Proof.
-  induction Γ in ξ |- *.
-  - reflexivity.
-  - cbn. eauto.
-Qed.
-
-(* TODO MOVE *)
-Lemma inst_equations_prop Σ Ξ ξ Ξ' P :
-  inst_equations Σ Ξ ξ Ξ' →
-  (∀ u v, Σ ;; Ξ ⊢ u ≡ v → P u v) →
-  inst_equations_ P ξ Ξ'.
-Proof.
-  intros h ih.
-  intros x rl hx. specialize (h _ _ hx).
-  cbn in *. intuition eauto.
-Qed.
-
-Lemma inst_typing_impl conv conv' typ typ' ξ Ξ :
-  inst_typing_ conv typ ξ Ξ →
-  (∀ u v, conv u v → conv' u v) →
-  (∀ t A, typ t A → typ' t A) →
-  inst_typing_ conv' typ' ξ Ξ.
-Proof.
-  intros h Xconv Xtyp.
-  induction h; constructor; eauto.
-Qed.
-
-Lemma inst_typing_ren0 Σ Ξ Δ Γ ρ ξ Ξ' :
-  rtyping Δ ρ Γ →
-  inst_typing_ (λ u v, ∀ ρ, Σ ;; Ξ ⊢ ρ ⋅ u ≡ ρ ⋅ v) (λ t A,
-    ∀ Δ ρ, rtyping Δ ρ Γ → Σ ;; Ξ | Δ ⊢ ρ ⋅ t : ρ ⋅ A
-  ) ξ Ξ' →
-  inst_typing Σ Ξ Δ (ren_instance ρ ξ) Ξ'.
-Proof.
-  intros hρ ih.
-  induction ih as [|??? ihh iihh m lhs rhs hl hhl hr hhr ih |???? ihh iihh hA hhA ih ].
-  - constructor.
-  - rewrite map_app. cbn. constructor; auto.
-    rewrite liftn_ren_instance.
-    fold m in hl, hr, ih |- *.
-    specialize ih with (ρ := uprens m ρ).
-    unfold lhs, rhs in ih.
-    rewrite 2!ren_inst in ih.
-    rewrite 2!scoped_ren in ih. 2,3: eassumption.
-    intuition eauto.
-  - rewrite map_app. cbn. constructor; auto.
-    specialize (ih _ _ hρ).
-    eapply meta_conv.
-    + eauto.
-    + rewrite !ren_inst. f_equal.
-      apply closed_ren. assumption.
-Qed.
-
-Lemma inst_typing_ren Σ Ξ Δ Γ ρ ξ Ξ' :
-  rtyping Δ ρ Γ →
-  inst_typing Σ Ξ Γ ξ Ξ' →
-  inst_typing_ (conversion Σ Ξ) (λ t A,
-    ∀ Δ ρ, rtyping Δ ρ Γ → Σ ;; Ξ | Δ ⊢ ρ ⋅ t : ρ ⋅ A
-  ) ξ Ξ' →
-  inst_typing Σ Ξ Δ (ren_instance ρ ξ) Ξ'.
-Proof.
-  intros ? H IH.
-  eapply inst_typing_ren0; eauto.
-  eapply inst_typing_impl with (1 := IH); eauto.
-  intros. now apply conv_ren.
-Qed.
-
-Lemma typing_ren :
-  ∀ Σ Ξ Γ Δ ρ t A,
+Lemma styping_ren :
+  ∀ Γ Δ ρ t A,
     rtyping Δ ρ Γ →
-    Σ ;; Ξ | Γ ⊢ t : A →
-    Σ ;; Ξ | Δ ⊢ ρ ⋅ t : ρ ⋅ A.
+    Γ ⊢ t : A →
+    Δ ⊢ ρ ⋅ t : ρ ⋅ A.
 Proof.
-  intros Σ Ξ Γ Δ ρ t A hρ ht.
-  induction ht using typing_ind in Δ, ρ, hρ |- *.
+  intros Γ Δ ρ t A hρ ht.
+  induction ht using styping_ind in Δ, ρ, hρ |- *.
   all: try solve [ rasimpl ; econstructor ; eauto using rtyping_up ].
-  - rasimpl. eapply hρ in H as [B [? eB]].
-    rasimpl in eB. rewrite eB.
-    econstructor. eassumption.
-  - rasimpl. rasimpl in IHht1. rasimpl in IHht4.
-    eapply meta_conv. 1: econstructor. all: eauto.
-    1:{ eauto using rtyping_up. }
-    rasimpl. reflexivity.
-  - rasimpl. eapply meta_conv. 1: econstructor.
-    + eassumption.
-    + eapply inst_typing_ren. all: eassumption.
-    + assumption.
-    + rewrite ren_inst. f_equal.
-      symmetry. apply closed_ren. assumption.
-  - rasimpl. rewrite closed_ren. 2: assumption.
-    econstructor. all: assumption.
-  - rasimpl. rasimpl in IHht2.
+  all: rasimpl.
+  2-5: rasimpl in IHht1; rasimpl in IHht4.
+  2-5: assert (((0 .: ρ >> S) ⋅ B) <[ (ρ ⋅ u)..] = B <[ ρ ⋅ u .: ρ >> var])
+       as <- by now rasimpl.
+  - eapply hρ in H as [B [? eB]].
+    rewrite eB. now econstructor.
+  - econstructor. all: eauto.
+    left. eauto using rtyping_up.
+  - econstructor. all: eauto.
+    right. eauto using rtyping_up.
+  - econstructor. all: eauto.
+    left. eauto using rtyping_up.
+  - econstructor. all: eauto.
+    right. eauto using rtyping_up.
+  - rasimpl in IHht2.
     econstructor. all: eauto.
-    eapply conv_ren. all: eassumption.
+    now apply conv_ren.
+  - rasimpl in IHht2.
+    econstructor. all: eauto.
+    now apply conv_ren.
 Qed.
 
 (** Reproving [ext_term] but with scoping assumption *)
@@ -869,18 +433,8 @@ Proof.
     cbn in * ; apply andb_prop in h ;
     f_equal ; intuition eauto using eq_subst_on_up
   ].
-  - cbn. apply e. cbn - ["<?"] in h. rewrite Nat.ltb_lt in h. assumption.
-  - cbn in *. f_equal.
-    apply map_ext_All.
-    apply forallb_All in h. move h at top.
-    eapply All_prod in h. 2: eassumption.
-    eapply All_impl. 2: eassumption. clear - e.
-    cbn. intros o [h1 h2].
-    apply option_map_ext_onSomeT.
-    apply onSomeb_onSome, onSome_onSomeT in h2.
-    eapply onSomeT_prod in h1. 2: eassumption.
-    eapply onSomeT_impl. 2: eassumption. clear - e.
-    cbn. intros t [h1 h2]. eauto.
+  cbn. apply e. cbn - ["<?"] in h.
+  now rewrite Nat.ltb_lt in h.
 Qed.
 
 (** Corollary: every substitution acts like a list of terms
@@ -924,15 +478,15 @@ Qed.
 
 (** Substitution preserves typing *)
 
-Inductive styping Σ Ξ (Γ : ctx) (σ : nat → term) : ctx → Prop :=
-| type_nil : styping Σ Ξ Γ σ ∙
+Inductive σtyping (Γ : ctx) (σ : nat → term) : ctx → Prop :=
+| type_nil : σtyping Γ σ ∙
 | type_cons Δ A :
-    styping Σ Ξ Γ (S >> σ) Δ →
-    Σ ;; Ξ | Γ ⊢ σ 0 : A <[ S >> σ ] →
-    styping Σ Ξ Γ σ (Δ ,, A).
+    σtyping Γ (S >> σ) Δ →
+    Γ ⊢ σ 0 : A <[ S >> σ ] →
+    σtyping Γ σ (Δ ,, A).
 
-#[export] Instance styping_morphism Σ Ξ :
-  Proper (eq ==> pointwise_relation _ eq ==> eq ==> iff) (styping Σ Ξ).
+#[export] Instance σtyping_morphism :
+  Proper (eq ==> pointwise_relation _ eq ==> eq ==> iff)σtyping.
 Proof.
   intros Γ ? <- σ σ' e Δ ? <-.
   revert σ σ' e. wlog_iff. intros σ σ' e h.
@@ -940,264 +494,61 @@ Proof.
   - constructor.
   - constructor.
     + apply ih. intros n. apply e.
-    + rewrite <- e. eapply meta_conv. 1: eassumption.
-      apply ext_term. intro. apply e.
+    + rewrite <- e.
+      assert (A <[ S >> σ] = A <[ S >> σ']) as <-.
+      { apply ext_term. intro. apply e. }
+      assumption.
 Qed.
 
-Lemma autosubst_simpl_styping :
-  ∀ Σ Ξ Γ Δ r s,
+Lemma autosubst_simpl_σtyping :
+  ∀ Γ Δ r s,
     SubstSimplification r s →
-    styping Σ Ξ Γ r Δ ↔ styping Σ Ξ Γ s Δ.
+    σtyping Γ r Δ ↔ σtyping Γ s Δ.
 Proof.
-  intros Σ Ξ Γ Δ r s H.
-  apply styping_morphism. 1,3: reflexivity.
+  intros Γ Δ r s H.
+  apply σtyping_morphism.
+  1,3: reflexivity.
   apply H.
 Qed.
 
-#[export] Hint Rewrite -> autosubst_simpl_styping : rasimpl_outermost.
+#[export] Hint Rewrite -> autosubst_simpl_σtyping : rasimpl_outermost.
 
-Lemma styping_weak Σ Ξ Γ Δ σ A :
-  styping Σ Ξ Γ σ Δ →
-  styping Σ Ξ (Γ,, A) (σ >> ren_term S) Δ.
+Lemma σtyping_weak Γ Δ σ A :
+  σtyping Γ σ Δ →
+  σtyping (Γ,, A) (σ >> ren_term S) Δ.
 Proof.
   intros h.
   induction h.
   - constructor.
   - constructor.
     + assumption.
-    + eapply meta_conv.
-      * eapply typing_ren. 2: eassumption.
-        apply rtyping_S.
-      * rasimpl. reflexivity.
+    + assert (S ⋅ A0 <[ S >> σ] = A0 <[ S >> (σ >> ren_term S)]) as <- by now rasimpl.
+      eapply styping_ren. 2: eassumption.
+      apply rtyping_S.
 Qed.
 
-Lemma styping_up Σ Ξ Γ Δ A σ :
-  styping Σ Ξ Γ σ Δ →
-  styping Σ Ξ (Γ ,, A <[ σ ]) (up_term σ) (Δ,, A).
+Lemma σtyping_up Γ Δ A σ :
+  σtyping Γ σ Δ →
+  σtyping (Γ ,, A <[ σ ]) (up_term σ) (Δ,, A).
 Proof.
   intros h.
   constructor.
-  - rasimpl. apply styping_weak. assumption.
-  - rasimpl. eapply meta_conv.
-    + econstructor. cbn. reflexivity.
-    + rasimpl. reflexivity.
+  - rasimpl. now apply σtyping_weak.
+  - rasimpl.
+    assert (Init.Nat.add 1 ⋅ A <[ σ] = A <[ σ >> ren_term S]) as <- by now rasimpl.
+    now econstructor.
 Qed.
 
-Lemma lift_liftn n ξ :
-  lift_instance (liftn n ξ) = liftn (S n) ξ.
-Proof.
-  rewrite ren_instance_comp. reflexivity.
-Qed.
-
-(**
-
-  Note: the condition is weird, because we can just use [trunc] to make it work
-  for any [m]. The fact that we're free to choose [m] suggests there is a better
-  lemma to be had.
-
-*)
-
-Lemma subst_inst σ ξ t n m :
-  (∀ k, σ (m + k) = var (n + k)) →
-  inst (liftn n ξ) (t <[ σ ]) =
-  (inst (liftn m ξ) t) <[ σ >> inst (liftn n ξ) ].
-Proof.
-  intro hσ.
-  induction t using term_rect in n, m, σ, hσ, ξ |- *.
-  all: try solve [ cbn ; f_equal ; eauto ].
-  - cbn. f_equal. 1: eauto.
-    rewrite lift_liftn. rewrite IHt2 with (m := S m).
-    2:{ intro. cbn. core.unfold_funcomp. rewrite hσ. reflexivity. }
-    rasimpl. rewrite lift_liftn.
-    apply ext_term.
-    intro. core.unfold_funcomp. cbn.
-    destruct x.
-    + cbn. reflexivity.
-    + cbn. repeat core.unfold_funcomp.
-      rewrite ren_inst.
-      rewrite lift_liftn. reflexivity.
-  - cbn. f_equal. 1: eauto.
-    rewrite lift_liftn. rewrite IHt2 with (m := S m).
-    2:{ intro. cbn. core.unfold_funcomp. rewrite hσ. reflexivity. }
-    rasimpl. rewrite lift_liftn.
-    apply ext_term.
-    intro. core.unfold_funcomp. cbn.
-    destruct x.
-    + cbn. reflexivity.
-    + cbn. repeat core.unfold_funcomp.
-      rewrite ren_inst.
-      rewrite lift_liftn. reflexivity.
-  - cbn. f_equal.
-    rewrite !map_map. apply map_ext_All.
-    eapply All_impl. 2: eassumption.
-    intros o ho. change @core.option_map with @option_map.
-    rewrite !option_map_option_map. apply option_map_ext_onSomeT.
-    eapply onSomeT_impl. 2: eassumption.
-    eauto.
-  - cbn. rewrite !iget_ren. rasimpl.
-    rewrite rinstInst'_term.
-    apply ext_term. intro k.
-    unfold core.funcomp.
-    rewrite hσ. cbn. reflexivity.
-Qed.
-
-Notation subst_instance σ ξ :=
-  (map_instance (subst_term σ) ξ).
-
-Lemma iget_subst σ ξ x :
-  iget (subst_instance σ ξ) x = (iget ξ x) <[ σ ].
-Proof.
-  unfold iget.
-  rewrite nth_error_map. destruct nth_error as [ [] |]. all: reflexivity.
-Qed.
-
-Lemma subst_inst_scoped σ ξ t k :
-  scoped k t = true →
-  (∀ n, n < k → σ n = var n) →
-  (inst ξ t) <[ σ ] = inst (subst_instance σ ξ) t.
-Proof.
-  intros h hσ.
-  induction t using term_rect in k, h, σ, hσ, ξ |- *.
-  all: try solve [ cbn ; f_equal ; eauto ].
-  - cbn - ["<?"] in *. apply Nat.ltb_lt in h. auto.
-  - cbn in *. apply andb_prop in h as [].
-    f_equal. 1: eauto.
-    erewrite IHt2. 2: eassumption.
-    2:{
-      intros [] h. 1: reflexivity.
-      rasimpl. cbn. core.unfold_funcomp. rewrite hσ. 2: lia.
-      reflexivity.
-    }
-    f_equal.
-    rewrite !map_map. apply map_ext. intro l.
-    rewrite !option_map_option_map. apply option_map_ext. intro t.
-    rasimpl. reflexivity.
-  - cbn in *. apply andb_prop in h as [].
-    f_equal. 1: eauto.
-    erewrite IHt2. 2: eassumption.
-    2:{
-      intros [] h. 1: reflexivity.
-      rasimpl. cbn. core.unfold_funcomp. rewrite hσ. 2: lia.
-      reflexivity.
-    }
-    f_equal.
-    rewrite !map_map. apply map_ext. intro l.
-    rewrite !option_map_option_map. apply option_map_ext. intro o.
-    rasimpl. reflexivity.
-  - cbn in *. apply andb_prop in h as [].
-    f_equal. all: eauto.
-  - cbn in *. f_equal.
-    rewrite map_map. apply map_ext_All.
-    apply forallb_All in h. move h at top.
-    eapply All_prod in h. 2: eassumption.
-    eapply All_impl. 2: eassumption. clear - hσ.
-    cbn. intros o [h1 h2].
-    change @core.option_map with option_map.
-    rewrite option_map_option_map. apply option_map_ext_onSomeT.
-    apply onSomeb_onSome, onSome_onSomeT in h2.
-    eapply onSomeT_prod in h1. 2: eassumption.
-    eapply onSomeT_impl. 2: eassumption. clear - hσ.
-    cbn. intros t [h1 h2]. eauto.
-  - cbn. symmetry. apply iget_subst.
-Qed.
-
-Corollary subst_inst_closed σ ξ t :
-  closed t = true →
-  (inst ξ t) <[ σ ] = inst (subst_instance σ ξ) t.
-Proof.
-  intro h.
-  eapply subst_inst_scoped.
-  - eassumption.
-  - lia.
-Qed.
-
-Corollary subst_inst_ups σ ξ t k :
-  scoped k t = true →
-  (inst ξ t) <[ ups k σ ] = inst (subst_instance (ups k σ) ξ) t.
-Proof.
-  intros h.
-  eapply subst_inst_scoped. 1: eassumption.
-  intros n hn.
-  induction k as [| k ih] in n, hn |- *. 1: lia.
-  cbn. destruct n.
-  - reflexivity.
-  - cbn. unfold core.funcomp. rewrite ih. 2: lia.
-    reflexivity.
-Qed.
-
-Lemma subst_instance_ext σ θ ξ :
-  (∀ n, σ n = θ n) →
-  subst_instance σ ξ = subst_instance θ ξ.
-Proof.
-  intros h.
-  apply map_ext. intro.
-  apply option_map_ext. intro.
-  apply ext_term. assumption.
-Qed.
-
-Lemma ren_subst_instance ρ σ ξ :
-  ren_instance ρ (subst_instance σ ξ) = subst_instance (σ >> (ren_term ρ)) ξ.
-Proof.
-  rewrite map_map. apply map_ext. intro.
-  rewrite option_map_option_map. apply option_map_ext. intro.
-  rasimpl. reflexivity.
-Qed.
-
-Lemma subst_ren_instance ρ σ ξ :
-  subst_instance σ (ren_instance ρ ξ) = subst_instance (ρ >> σ) ξ.
-Proof.
-  rewrite map_map. apply map_ext. intro.
-  rewrite option_map_option_map. apply option_map_ext. intro.
-  rasimpl. reflexivity.
-Qed.
-
-Corollary liftn_subst_instance n σ ξ :
-  liftn n (subst_instance σ ξ) = subst_instance (ups n σ) (liftn n ξ).
-Proof.
-  rewrite subst_ren_instance. rewrite ren_subst_instance.
-  apply subst_instance_ext. intro m.
-  unfold core.funcomp.
-  induction n as [| n ih] in m, σ |- *.
-  - cbn. rasimpl. reflexivity.
-  - cbn. unfold core.funcomp. rewrite <- ih.
-    rasimpl. reflexivity.
-Qed.
-
-Lemma inst_equations_subst_ih Σ Ξ σ ξ Ξ' :
-  inst_equations Σ Ξ ξ Ξ' →
-  inst_equations_ (λ u v, ∀ σ, Σ ;; Ξ ⊢ u <[ σ ] ≡ v <[ σ ]) ξ Ξ' →
-  inst_equations Σ Ξ (subst_instance σ ξ) Ξ'.
-Proof.
-  intros h ih.
-  intros x rl hx m. specialize (ih _ _ hx).
-  cbn in ih. fold m in ih. destruct ih as (e & hl & hr & ih).
-  specialize ih with (σ := ups m σ).
-  cbn.
-  rewrite !liftn_subst_instance.
-  erewrite 2!subst_inst_ups in ih. 2,3: eassumption.
-  rewrite nth_error_map. rewrite e.
-  intuition eauto.
-Qed.
-
-Lemma conv_subst Σ Ξ σ u v :
-  Σ ;; Ξ ⊢ u ≡ v →
-  Σ ;; Ξ ⊢ u <[ σ ] ≡ v <[ σ ].
+Lemma conv_subst σ u v :
+  u ≡ v →
+  u <[ σ ] ≡ v <[ σ ].
 Proof.
   intros h.
   induction h using conversion_ind in σ |- *.
   all: try solve [ rasimpl ; econstructor ; eauto ].
-  - rasimpl. eapply meta_conv_trans_r. 1: econstructor.
-    rasimpl. reflexivity.
-  - cbn. eapply meta_conv_trans_r.
-    1:{ econstructor. 1,3: eassumption. 1: eauto using inst_equations_subst_ih. }
-    symmetry. apply subst_inst_closed. assumption.
-  - cbn. constructor.
-    apply Forall2_map_l, Forall2_map_r.
-    eapply Forall2_impl. 2: eassumption.
-    intros l l' h.
-    apply option_rel_map_l, option_rel_map_r.
-    eapply option_rel_impl. 2: eassumption.
-    cbn. auto.
+  - assert ((t <[ (var 0) .: σ >> ren_term S]) <[ (u <[ σ])..] = (t <[ u..]) <[ σ])
+    as <- by now rasimpl.
+    econstructor.
 Qed.
 
 Lemma scoped_subst σ k t :
@@ -1214,21 +565,9 @@ Proof.
     f_equal ;
     eauto
   ].
-  - cbn - ["<?"] in *.
-    apply ups_below.
-    apply Nat.ltb_lt. assumption.
-  - cbn in *. f_equal.
-    rewrite <- map_id. apply map_ext_All.
-    apply forallb_All in h. move h at top.
-    eapply All_prod in h. 2: eassumption.
-    eapply All_impl. 2: eassumption. clear.
-    cbn. intros ? [h1 h2].
-    change @core.option_map with option_map.
-    apply option_map_id_onSomeT.
-    apply onSomeb_onSome, onSome_onSomeT in h2.
-    eapply onSomeT_prod in h1. 2: eassumption.
-    eapply onSomeT_impl. 2: eassumption. clear.
-    cbn. intros t [h1 h2]. eauto.
+  cbn - ["<?"] in *.
+  apply ups_below.
+  apply Nat.ltb_lt. assumption.
 Qed.
 
 Corollary closed_subst σ t :
@@ -1237,35 +576,6 @@ Corollary closed_subst σ t :
 Proof.
   intros h.
   eapply scoped_subst in h. eauto.
-Qed.
-
-Lemma subst_instance_id ξ :
-  subst_instance ids ξ = ξ.
-Proof.
-  rewrite <- map_id. apply map_ext. intro.
-  rewrite <- option_map_id. apply option_map_ext. intro.
-  rasimpl. reflexivity.
-Qed.
-
-Lemma closed_subst_instance σ ξ :
-  closed_instance ξ = true →
-  subst_instance σ ξ = ξ.
-Proof.
-  intros h.
-  etransitivity. 2: apply subst_instance_id.
-  apply map_ext_All. eapply All_impl.
-  2:{ apply forallb_All. eassumption. }
-  cbn. intros ? ho%onSomeb_onSome%onSome_onSomeT.
-  apply option_map_ext_onSomeT. eapply onSomeT_impl. 2: eassumption.
-  cbn. rasimpl. apply closed_subst.
-Qed.
-
-Lemma closed_lift_instance ξ :
-  closed_instance ξ = true →
-  closed_instance (lift_instance ξ) = true.
-Proof.
-  intro h.
-  rewrite closed_ren_instance. all: assumption.
 Qed.
 
 Lemma scoped_upwards k l t :
@@ -1280,15 +590,7 @@ Proof.
     cbn in * ; rewrite Bool.andb_true_iff in * ;
     intuition eauto with arith
   ].
-  - cbn - ["<?"] in *. rewrite Nat.ltb_lt in *. lia.
-  - cbn in *. apply All_forallb. apply forallb_All in ht.
-    move ht at top. eapply All_prod in ht. 2: eassumption.
-    eapply All_impl. 2: eassumption.
-    cbn. intros ? [h1 h2]. apply onSomeb_onSome, onSomeT_onSome.
-    apply onSomeb_onSome, onSome_onSomeT in h2.
-    eapply onSomeT_prod in h1. 2: eassumption.
-    eapply onSomeT_impl. 2: eassumption.
-    cbn. intros ? []. eauto.
+  cbn - ["<?"] in *. rewrite Nat.ltb_lt in *. lia.
 Qed.
 
 Lemma uprens_below k ρ n :
@@ -1340,16 +642,6 @@ Proof.
     change (upRen_term_term (uprens m ?ρ)) with (uprens (S m) ρ).
     change (S (m + k + l)) with (S m + k + l).
     eauto.
-  - cbn in *. apply forallb_All in h. move h at top.
-    eapply All_prod in h. 2: eassumption.
-    apply All_forallb. apply All_map. eapply All_impl. 2: eassumption.
-    clear.
-    cbn. intros σ [h1 h2].
-    apply onSomeb_onSome, onSomeT_onSome. apply onSomeT_map.
-    apply onSomeb_onSome, onSome_onSomeT in h2.
-    eapply onSomeT_prod in h1. 2: eassumption.
-    eapply onSomeT_impl. 2: eassumption. clear.
-    cbn. intros t [h1 h2]. eauto.
 Qed.
 
 Lemma scoped_lift k l t :
@@ -1361,875 +653,94 @@ Proof.
   assumption.
 Qed.
 
-Lemma scoped_inst k l ξ t :
-  scoped_instance l ξ = true →
-  scoped k t = true →
-  scoped (k + l) (inst (liftn k ξ) t) = true.
-Proof.
-  intros hξ ht.
-  induction t using term_rect in k, l, ξ, ht, hξ |- *.
-  all: try solve [ cbn ; eauto ].
-  all: try solve [
-    cbn in * ; rewrite Bool.andb_true_iff in * ;
-    (* rewrite Nat.ltb_lt in * ; *)
-    intuition eauto with arith
-  ].
-  - cbn - ["<=?"] in *.
-    rewrite Nat.ltb_lt in *. eauto with arith.
-  - cbn in *. rewrite Bool.andb_true_iff in *.
-    intuition eauto.
-    rewrite lift_liftn. change (S (k + l)) with (S k + l). eauto.
-  - cbn in *. rewrite Bool.andb_true_iff in *.
-    intuition eauto.
-    rewrite lift_liftn. change (S (k + l)) with (S k + l). eauto.
-  - cbn in *. apply forallb_All in ht. move ht at top.
-    eapply All_prod in ht. 2: eassumption.
-    apply All_forallb. apply All_map. eapply All_impl. 2: eassumption.
-    clear - hξ.
-    cbn. intros o [h1 h2].
-    apply onSomeb_onSome, onSomeT_onSome. apply onSomeT_map.
-    apply onSomeb_onSome, onSome_onSomeT in h2.
-    eapply onSomeT_prod in h1. 2: eassumption.
-    eapply onSomeT_impl. 2: eassumption. clear - hξ.
-    cbn. intros t [h1 h2]. eauto.
-  - cbn. rewrite iget_ren. unfold iget.
-    destruct nth_error as [[t|] |] eqn: hx. 2,3: reflexivity.
-    apply nth_error_In in hx.
-    rewrite forallb_forall in hξ. specialize hξ with (1 := hx).
-    eapply scoped_lift. assumption.
-Qed.
-
-Corollary scoped_inst_closed k ξ t :
-  scoped_instance k ξ = true →
-  closed t = true →
-  scoped k (inst ξ t) = true.
-Proof.
-  intros hξ ht.
-  eapply scoped_inst in hξ. 2: eassumption.
-  cbn in hξ. rewrite ren_instance_id in hξ. assumption.
-Qed.
-
-Corollary closed_inst ξ t :
-  closed_instance ξ = true →
-  closed t = true →
-  closed (inst ξ t) = true.
-Proof.
-  intros hξ ht.
-  apply scoped_inst_closed. all: assumption.
-Qed.
-
-Lemma inst_typing_subst0 Σ Ξ Δ Γ σ ξ Ξ' :
-  styping Σ Ξ Δ σ Γ →
-  inst_typing_ (λ u v, ∀ σ, Σ ;; Ξ ⊢ u <[ σ ] ≡ v <[ σ ]) (λ t A,
-    ∀ Δ σ, styping Σ Ξ Δ σ Γ → Σ ;; Ξ | Δ ⊢ t <[ σ ] : A <[ σ ]
-  ) ξ Ξ' →
-  inst_typing Σ Ξ Δ (subst_instance σ ξ) Ξ'.
-Proof.
-  intros hρ ih.
-  induction ih as [|??? ihh iihh m lhs rhs hl hhl hr hhr ih |???? ihh iihh hA hhA ih].
-  - constructor.
-  - rewrite map_app. cbn. constructor; auto.
-    rewrite liftn_subst_instance.
-    fold m in hl, hr, ih |- *.
-    specialize ih with (σ := ups m σ).
-    unfold lhs, rhs in ih.
-    erewrite 2!subst_inst_ups in ih. 2,3: eassumption.
-    intuition eauto.
-  - rewrite map_app. cbn. constructor; auto.
-    specialize (ih _ _ hρ).
-    eapply meta_conv.
-    + eauto.
-    + apply subst_inst_closed. assumption.
-Qed.
-
-Lemma inst_typing_subst Σ Ξ Δ Γ σ ξ Ξ' :
-  styping Σ Ξ Δ σ Γ →
-  inst_typing Σ Ξ Γ ξ Ξ' →
-  inst_typing_ (conversion Σ Ξ) (λ t A,
-    ∀ Δ σ, styping Σ Ξ Δ σ Γ → Σ ;; Ξ | Δ ⊢ t <[ σ ] : A <[ σ ]
-  ) ξ Ξ' →
-  inst_typing Σ Ξ Δ (subst_instance σ ξ) Ξ'.
-Proof.
-  intros ? H IH.
-  eapply inst_typing_subst0; eauto.
-  eapply inst_typing_impl with (1 := IH); eauto.
-  intros. now apply conv_subst.
-Qed.
-
-Lemma typing_subst Σ Ξ Γ Δ σ t A :
-  styping Σ Ξ Δ σ Γ →
-  Σ ;; Ξ | Γ ⊢ t : A →
-  Σ ;; Ξ | Δ ⊢ t <[ σ ] : A <[ σ ].
+Lemma styping_subst Γ Δ σ t A :
+  σtyping Δ σ Γ →
+  Γ ⊢ t : A →
+  Δ ⊢ t <[ σ ] : A <[ σ ].
 Proof.
   intros hσ ht.
-  induction ht using typing_ind in Δ, σ, hσ |- *.
-  all: try solve [ rasimpl ; econstructor ; eauto using styping_up ].
+  induction ht using styping_ind in Δ, σ, hσ |- *.
+  all: try solve [ rasimpl ; econstructor ; eauto using σtyping_up ].
   - rasimpl.
     induction hσ in x, H |- *. 1: destruct x ; discriminate.
     destruct x.
     + cbn in H. inversion H. subst. assumption.
     + apply IHhσ. assumption.
-  - rasimpl. eapply meta_conv.
-    + cbn in *. econstructor ; eauto using styping_up.
-    + rasimpl. reflexivity.
-  - cbn. eapply meta_conv.
-    + econstructor. 1,3: eassumption.
-      eapply inst_typing_subst. all: eassumption.
-    + symmetry. apply subst_inst_closed. assumption.
-  - cbn. rewrite closed_subst. 2: assumption.
-    econstructor. all: eassumption.
+  - assert ((B <[ up_term_term σ]) <[ (u <[ σ])..] = (B <[ u..]) <[ σ])
+      as <- by now rasimpl.
+    cbn in *. econstructor ; eauto using σtyping_up.
+  - assert ((B <[ up_term_term σ]) <[ (u <[ σ])..] = (B <[ u..]) <[ σ])
+      as <- by now rasimpl.
+    cbn in *. econstructor ; eauto using σtyping_up.
+  - assert ((B <[ up_term_term σ]) <[ (u <[ σ])..] = (B <[ u..]) <[ σ])
+      as <- by now rasimpl.
+    cbn in *. econstructor ; eauto using σtyping_up.
+  - assert ((B <[ up_term_term σ]) <[ (u <[ σ])..] = (B <[ u..]) <[ σ])
+      as <- by now rasimpl.
+    cbn in *. econstructor ; eauto using σtyping_up.
+  - econstructor. 1,3: eauto.
+    eapply conv_subst. eassumption.
   - econstructor. 1,3: eauto.
     eapply conv_subst. eassumption.
 Qed.
 
-(** Instances preserve conversion and typing *)
-
-Lemma iscoped_inst_ext ξ ξ' Ξ n t :
-  iscope Ξ t →
-  (forall n a, ictx_get Ξ n = Some (Assm a) -> nth_error ξ n = nth_error ξ' n) →
-  inst (liftn n ξ) t = inst (liftn n ξ') t.
-Proof.
-  intros h hξ.
-  induction t using term_rect in n, h |- *.
-  all: try solve [ depelim h ; cbn ; eauto ].
-  all: try solve [ depelim h ; cbn ; f_equal; eauto ].
-  - depelim h. cbn. f_equal; eauto.
-    rewrite !lift_liftn. auto.
-  - depelim h. cbn. f_equal; eauto.
-    rewrite !lift_liftn. auto.
-  - depelim h. cbn. f_equal.
-    induction X; inversion H; subst.
-    + reflexivity.
-    + cbn. f_equal; auto. depelim H2; try reflexivity. cbn. f_equal. cbn in p. auto.
-  - cbn. depelim h.
-    specialize (hξ _ _ H).
-    unfold iget. rewrite !nth_error_map.
-    rewrite hξ. reflexivity.
-Qed.
-
-Lemma inst_typing_equations Σ Ξ P' ξ Ξ' :
-  inst_typing_ (conversion Σ Ξ) P' ξ Ξ' →
-  inst_equations_ (conversion Σ Ξ) ξ Ξ'.
-Proof.
-  intros H.
-  assert (Xa : ∀ x (n : aref) (a : term),
-    ictx_get (skipn (Datatypes.length Ξ' - x) Ξ') n = Some (Assm a)
-    → nth_error ξ n = nth_error (firstn x ξ) n).
-  { intros ??? H0.
-    assert (H1 : n < length (rev (skipn (length Ξ' - x) Ξ'))). { apply nth_error_Some. unfold ictx_get in H0. rewrite H0. now intro. }
-    clear H0.
-    rewrite nth_error_firstn.
-    destruct (Nat.ltb_spec n x); auto. rewrite length_rev, length_skipn in H1. lia.
-  }
-  intros x rl hx m lhs rhs.
-  eapply inst_typing_ictx_get_comp in hx as h; eauto.
-  destruct h as (?&?&?&?&?&?).
-  split; auto. split; auto. split; auto.
-  unfold lhs, rhs.
-  erewrite iscoped_inst_ext with (t := cr_pat rl), iscoped_inst_ext with (t := cr_rep rl); eauto.
-Qed.
-
-Lemma inst_typing_iget Σ Ξ Γ ξ Ξ' :
-  inst_typing Σ Ξ Γ ξ Ξ' →
-  inst_iget Σ Ξ Γ ξ Ξ'.
-Proof.
-  intros H n t hx.
-  assert (Xa : ∀ x (n' : aref) (a : term),
-    ictx_get (skipn (Datatypes.length Ξ' - x) Ξ') n' = Some (Assm a)
-    → nth_error (firstn x ξ) n' = nth_error ξ n').
-  { intros ??? H0.
-    assert (H1 : n' < length (rev (skipn (length Ξ' - x) Ξ'))). { apply nth_error_Some. unfold ictx_get in H0. rewrite H0. now intro. }
-    clear H0.
-    rewrite nth_error_firstn.
-    destruct (Nat.ltb_spec n' x); auto. rewrite length_rev, length_skipn in H1. lia.
-  }
-  eapply inst_typing_ictx_get_assm in hx as h; eauto.
-  destruct h as (?&?&?& e & h).
-  split; auto.
-  unfold iget. rewrite e.
-  replace (inst ξ t) with (inst (firstn n ξ) t); auto.
-  rewrite <- (ren_instance_id ξ). rewrite ren_instance_id at 1.
-  rewrite <- (ren_instance_id (firstn n ξ)).
-  eapply iscoped_inst_ext with (n := 0); eauto.
-Qed.
-
-
-Lemma nth_error_ctx_inst ξ Γ x :
-  nth_error (ctx_inst ξ Γ) x =
-  option_map (inst (ren_instance (plus (length Γ - S x)) ξ)) (nth_error Γ x).
-Proof.
-  induction Γ in ξ, x |- *.
-  - cbn. rewrite nth_error_nil. reflexivity.
-  - destruct x as [| x].
-    + cbn. replace (length Γ - 0) with (length Γ) by lia.
-      reflexivity.
-    + cbn. eauto.
-Qed.
-
-Lemma ctx_inst_app ξ Γ Δ :
-  ctx_inst ξ (Γ ,,, Δ) = ctx_inst ξ Γ ,,, ctx_inst (liftn (length Γ) ξ) Δ.
-Proof.
-  induction Δ as [| A Δ ih] in Γ |- *.
-  - reflexivity.
-  - cbn. f_equal. 2: eauto.
-    rewrite liftn_liftn. rewrite length_app. reflexivity.
-Qed.
-
-Lemma inst_get ξ ξ' x :
-  inst ξ (iget ξ' x) = iget (inst_instance ξ ξ') x.
-Proof.
-  unfold iget. rewrite nth_error_map.
-  destruct nth_error as [[]|]. all: reflexivity.
-Qed.
-
-Lemma inst_inst ξ ξ' t :
-  inst ξ (inst ξ' t) = inst (inst_instance ξ ξ') t.
-Proof.
-  induction t using term_rect in ξ, ξ' |- *.
-  all: try solve [ cbn ; f_equal ; eauto ].
-  - cbn. f_equal. 1: eauto.
-    rewrite IHt2. f_equal.
-    rewrite !map_map. apply map_ext. intro o.
-    rewrite !option_map_option_map. apply option_map_ext. intro t.
-    symmetry. apply ren_inst.
-  - cbn. f_equal. 1: eauto.
-    rewrite IHt2. f_equal.
-    rewrite !map_map. apply map_ext. intro o.
-    rewrite !option_map_option_map. apply option_map_ext. intro t.
-    symmetry. apply ren_inst.
-  - cbn. f_equal.
-    rewrite !map_map. apply map_ext_All.
-    eapply All_impl. 2: eassumption.
-    intros o ho.
-    rewrite !option_map_option_map. apply option_map_ext_onSomeT.
-    eapply onSomeT_impl. 2: eassumption.
-    auto.
-  - cbn. apply inst_get.
-Qed.
-
-Lemma liftn_inst_instance n ξ ξ' :
-  liftn n (inst_instance ξ ξ') = inst_instance (liftn n ξ) (liftn n ξ').
-Proof.
-  rewrite !map_map. apply map_ext. intro.
-  rewrite !option_map_option_map. apply option_map_ext. intro.
-  rewrite ren_inst. reflexivity.
-Qed.
-
-Lemma ctx_inst_comp ξ ξ' Γ :
-  ctx_inst ξ (ctx_inst ξ' Γ) = ctx_inst (inst_instance ξ ξ') Γ.
-Proof.
-  induction Γ as [| A Γ ih].
-  - reflexivity.
-  - cbn. rewrite ih. f_equal. rewrite inst_inst. f_equal.
-    rewrite length_ctx_inst.
-    rewrite liftn_inst_instance. reflexivity.
-Qed.
-
-Lemma inst_equations_inst_ih Σ Ξ Ξ' Ξ'' k ξ ξ' :
-  inst_equations Σ Ξ ξ Ξ' →
-  inst_equations Σ Ξ' ξ' Ξ'' →
-  inst_equations_ (λ u v,
-    ∀ Ξ p ξ,
-      inst_equations Σ Ξ ξ Ξ' →
-      Σ ;; Ξ ⊢ inst (liftn p ξ) u ≡ inst (liftn p ξ) v
-  ) ξ' Ξ'' →
-  inst_equations Σ Ξ (inst_instance (liftn k ξ) ξ') Ξ''.
-Proof.
-  intros hξ h ih.
-  intros x rl hx m. specialize (ih _ _ hx) as (e & hl & hr & ih).
-  cbn in *. fold m in ih.
-  specialize ih with (1 := hξ) (p := m + k).
-  rewrite !inst_inst in ih.
-  rewrite liftn_inst_instance.
-  rewrite liftn_liftn.
-  rewrite nth_error_map, e. cbn.
-  intuition eauto.
-Qed.
-
-Lemma conv_inst Σ Ξ Ξ' k u v ξ :
-  inst_equations Σ Ξ ξ Ξ' →
-  Σ ;; Ξ' ⊢ u ≡ v →
-  let rξ := liftn k ξ in
-  Σ ;; Ξ ⊢ inst rξ u ≡ inst rξ v.
-Proof.
-  intros hξ h. cbn.
-  induction h using conversion_ind in Ξ, k, ξ, hξ |- *.
-  all: try solve [ cbn ; econstructor ; eauto ].
-  - cbn. rewrite subst_inst with (m := S k). 2: auto.
-    eapply meta_conv_trans_r. 1: constructor.
-    cbn. rewrite lift_liftn. apply ext_term. intros []. all: reflexivity.
-  - cbn. eapply meta_conv_trans_r.
-    1:{
-      eapply conv_unfold. 1,3: eassumption.
-      eauto using inst_equations_inst_ih.
-    }
-    rewrite inst_inst. reflexivity.
-  - erewrite ext_term_scoped. 3: eapply eq_subst_trunc. 2: eassumption.
-    erewrite (ext_term_scoped _ rhs).
-    3: eapply eq_subst_trunc. 2: eassumption.
-    erewrite 2!subst_inst. 2,3: eapply trunc_bounds.
-    eapply conv_subst. eapply hξ. eassumption.
-  - cbn. constructor. 1: eauto.
-    rewrite lift_liftn.
-    apply IHh2. assumption.
-  - cbn. constructor. 1: eauto.
-    rewrite lift_liftn.
-    apply IHh2. assumption.
-  - cbn. constructor.
-    apply Forall2_map_l, Forall2_map_r.
-    eapply Forall2_impl. 2: eassumption.
-    intros l l' h.
-    apply option_rel_map_l, option_rel_map_r.
-    eapply option_rel_impl. 2: eassumption.
-    cbn. auto.
-Qed.
-
-Corollary conv_inst_closed Σ Ξ Ξ' u v ξ :
-  inst_equations Σ Ξ ξ Ξ' →
-  Σ ;; Ξ' ⊢ u ≡ v →
-  Σ ;; Ξ ⊢ inst ξ u ≡ inst ξ v.
-Proof.
-  intros hξ h.
-  eapply conv_inst with (k := 0) in h. 2: eassumption.
-  cbn in h. rewrite ren_instance_id_ext in h. 2: auto.
-  assumption.
-Qed.
-
-Lemma inst_typing_inst0 Σ Ξ Γ ξ Ξ' Δ ξ' Ξ'' :
-  inst_typing Σ Ξ Δ ξ Ξ' →
-  let rξ := liftn (length Γ) ξ in
-  inst_typing_
-    (λ u v, ∀ p, Σ ;; Ξ ⊢ inst (liftn p ξ) u ≡ inst (liftn p ξ) v)
-    (λ t A, Σ ;; Ξ | Δ ,,, ctx_inst ξ Γ ⊢ inst rξ t : inst rξ A)
-    ξ' Ξ'' →
-  inst_typing Σ Ξ (Δ ,,, ctx_inst ξ Γ) (inst_instance rξ ξ') Ξ''.
-Proof.
-  intros hξ rξ ih. unfold rξ in *.
-  induction ih as [|??? ihh iihh m lhs rhs hl hhl hr hhr ih |???? ihh iihh hA hhA ih].
-  - constructor.
-  - rewrite map_app. cbn. constructor; auto.
-    fold m in hl, hr, ih |- *.
-    unfold lhs, rhs in ih.
-    specialize ih with (p := m + length Γ).
-    rewrite !inst_inst in ih.
-    rewrite liftn_inst_instance.
-    rewrite !liftn_liftn.
-    assumption.
-  - rewrite map_app. cbn. constructor; auto.
-    cbn in ih.
-    rewrite inst_inst in ih.
-    assumption.
-Qed.
-
-Lemma inst_typing_inst Σ Ξ Γ ξ Ξ' Δ ξ' Ξ'' :
-  inst_typing Σ Ξ Δ ξ Ξ' →
-  let rξ := liftn (length Γ) ξ in
-  inst_typing_
-    (conversion Σ Ξ')
-    (λ t A, Σ ;; Ξ | Δ ,,, ctx_inst ξ Γ ⊢ inst rξ t : inst rξ A)
-    ξ' Ξ'' →
-  inst_typing Σ Ξ (Δ ,,, ctx_inst ξ Γ) (inst_instance rξ ξ') Ξ''.
-Proof.
-  intros ? H IH.
-  eapply inst_typing_inst0; eauto.
-  eapply inst_typing_impl with (1 := IH); eauto.
-  intros. eapply conv_inst; eauto. eapply inst_typing_equations, H0; eauto.
-Qed.
-
-Lemma typing_inst Σ Ξ Ξ' Γ Δ t A ξ :
-  inst_typing Σ Ξ Δ ξ Ξ' →
-  Σ ;; Ξ' | Γ ⊢ t : A →
-  let rξ := liftn (length Γ) ξ in
-  Σ ;; Ξ | Δ ,,, ctx_inst ξ Γ ⊢ inst rξ t : inst rξ A.
-Proof.
-  intros hξ ht rξ.
-  induction ht using typing_ind in Ξ, Δ, ξ, rξ, hξ |- *.
-  all: try solve [ cbn ; econstructor ; eauto ].
-  - cbn. eapply meta_conv.
-    + econstructor. rewrite nth_error_app1.
-      2:{ rewrite length_ctx_inst. eapply nth_error_Some. congruence. }
-      rewrite nth_error_ctx_inst.
-      rewrite H. cbn. reflexivity.
-    + rewrite ren_inst. f_equal.
-      rewrite liftn_liftn.
-      apply ren_instance_ext.
-      cbn. intro.
-      pose proof (nth_error_Some Γ x) as e%proj1.
-      forward e by congruence.
-      lia.
-  - cbn. constructor. 1: eauto.
-    subst rξ. rewrite ren_instance_comp. apply IHht2. assumption.
-  - cbn. econstructor. 1: eauto.
-    + subst rξ. rewrite ren_instance_comp. apply IHht2. assumption.
-    + subst rξ. rewrite ren_instance_comp. apply IHht3. assumption.
-  - cbn. eapply meta_conv.
-    + cbn in *. econstructor. all: eauto.
-      subst rξ. rewrite ren_instance_comp. apply IHht4. assumption.
-    + rasimpl.
-      subst rξ. erewrite subst_inst with (m := S (length Γ)).
-      2:{ cbn. auto. }
-      rewrite lift_liftn.
-      apply ext_term. intros []. all: reflexivity.
-  - cbn. eapply meta_conv.
-    + econstructor. 1,3: eassumption.
-      eapply inst_typing_inst; eauto.
-      eapply inst_typing_impl; eauto.
-    + rewrite inst_inst. reflexivity.
-  - cbn. subst rξ. rewrite iget_ren.
-    eapply meta_conv.
-    + eapply typing_ren.
-      1:{ erewrite <- length_ctx_inst. eapply rtyping_add. }
-      eapply inst_typing_iget in hξ.
-      eapply hξ. eassumption.
-    + rewrite ren_inst. f_equal.
-      apply closed_ren. assumption.
-  - econstructor. 1,3: eauto.
-    eapply conv_inst. 2: eassumption.
-    eapply inst_typing_equations, hξ; eauto.
-Qed.
-
-Corollary typing_inst_closed Σ Ξ Ξ' Γ t A ξ :
-  inst_typing Σ Ξ Γ ξ Ξ' →
-  Σ ;; Ξ' | ∙ ⊢ t : A →
-  Σ ;; Ξ | Γ ⊢ inst ξ t : inst ξ A.
-Proof.
-  intros hξ h.
-  eapply typing_inst in h; eauto.
-  cbn in h.
-  rewrite ren_instance_id_ext in h. 2: auto.
-  assumption.
-Qed.
-
-Lemma conv_insts Σ Ξ t ξ ξ' :
-  Forall2 (option_rel (conversion Σ Ξ)) ξ ξ' →
-  Σ ;; Ξ ⊢ inst ξ t ≡ inst ξ' t.
-Proof.
-  intros hξ.
-  induction t using term_rect in ξ, ξ', hξ |- *.
-  all: try solve [ cbn ; ttconv ].
-  - cbn. eapply cong_Pi. 1: eauto.
-    eapply IHt2. eapply Forall2_map_l, Forall2_map_r.
-    eapply Forall2_impl. 2: eassumption.
-    intros.
-    eapply option_rel_map_l, option_rel_map_r.
-    eapply option_rel_impl. 2: eassumption.
-    intros. eapply conv_ren. eassumption.
-  - cbn. eapply cong_lam. 1: eauto.
-    eapply IHt2. eapply Forall2_map_l, Forall2_map_r.
-    eapply Forall2_impl. 2: eassumption.
-    intros.
-    eapply option_rel_map_l, option_rel_map_r.
-    eapply option_rel_impl. 2: eassumption.
-    intros. eapply conv_ren. eassumption.
-  - cbn. eapply cong_const.
-    eapply Forall2_map_l, Forall2_map_r.
-    eapply Forall2_diag. eapply All_Forall.
-    eapply All_impl. 2: eassumption.
-    intros.
-    eapply option_rel_map_l, option_rel_map_r.
-    eapply option_rel_diag. rewrite OnSome_onSome. apply onSomeT_onSome.
-    eapply onSomeT_impl. 2: eassumption.
-    cbn. intros. eauto.
-  - cbn. unfold iget. destruct (nth_error ξ _) as [o1 |] eqn:e1.
-    2:{
-      destruct (nth_error ξ' _) eqn:e2.
-      1:{
-        eapply nth_error_None in e1. eapply Forall2_length in hξ.
-        rewrite hξ in e1. rewrite <- nth_error_None in e1. congruence.
-      }
-      ttconv.
-    }
-    eapply Forall2_nth_error_l in e1 as e2. 2: eassumption.
-    destruct e2 as (o2 & e2 & h). rewrite e2.
-    destruct h. 1: ttconv.
-    assumption.
-Qed.
-
-Lemma cong_inst Σ Ξ u v ξ ξ' Ξ' :
-  inst_equations Σ Ξ ξ Ξ' →
-  Σ ;; Ξ' ⊢ u ≡ v →
-  Forall2 (option_rel (conversion Σ Ξ)) ξ ξ' →
-  Σ ;; Ξ ⊢ inst ξ u ≡ inst ξ' v.
-Proof.
-  intros hξ h hh.
-  eapply conv_trans.
-  - eapply conv_inst_closed. all: eassumption.
-  - eapply conv_insts. assumption.
-Qed.
-
-(** Extension environement weakening *)
-
-Lemma ictx_get_weak d Ξ M i :
-  ictx_get Ξ M = Some i →
-  ictx_get (d :: Ξ) M = Some i.
-Proof.
-  apply lvl_get_weak.
-Qed.
-
-Lemma conv_eweak Σ Ξ d u v :
-  Σ ;; Ξ ⊢ u ≡ v →
-  Σ ;; d :: Ξ ⊢ u ≡ v.
-Proof.
-  intros h. induction h using conversion_ind.
-  all: try solve [ econstructor ; eauto ].
-  econstructor. 2-3: eauto.
-  apply ictx_get_weak. eassumption.
-Qed.
-
-Lemma inst_equations_eweak Σ Ξ d ξ Ξ' :
-  inst_equations Σ Ξ ξ Ξ' →
-  inst_equations Σ (d :: Ξ) ξ Ξ'.
-Proof.
-  intros h.
-  intros x rl hx. specialize (h _ _ hx).
-  cbn in *. intuition eauto using conv_eweak.
-Qed.
-
-Lemma inst_iget_eweak Σ Ξ d Γ ξ Ξ' :
-  inst_iget Σ Ξ Γ ξ Ξ' →
-  inst_iget_ (λ Γ t A, Σ ;; d :: Ξ | Γ ⊢ t : A) Γ ξ Ξ' →
-  inst_iget Σ (d :: Ξ) Γ ξ Ξ'.
-Proof.
-  intros h ih.
-  intros x A hx. specialize (ih _ _ hx) as [? ih].
-  split. 1: assumption.
-  eauto.
-Qed.
-
-Lemma inst_typing_eweak_ Σ Ξ d Γ ξ Ξ' :
-  inst_typing_ (conversion Σ Ξ) (λ t A, Σ ;; d :: Ξ | Γ ⊢ t : A) ξ Ξ' →
-  inst_typing Σ (d :: Ξ) Γ ξ Ξ'.
-Proof.
-  induction 1; constructor; eauto.
-  now apply conv_eweak.
-Qed.
-
-Lemma typing_eweak Σ Ξ d Γ t A :
-  Σ ;; Ξ | Γ ⊢ t : A →
-  Σ ;; d :: Ξ | Γ ⊢ t : A.
-Proof.
-  intros h. induction h using typing_ind.
-  all: try solve [ econstructor ; eauto ].
-  - econstructor. 1,3: eauto.
-    eapply inst_typing_eweak_. all: eassumption.
-  - econstructor. 2: assumption.
-    eapply ictx_get_weak. assumption.
-  - econstructor. 1,3: eassumption.
-    eapply conv_eweak. assumption.
-Qed.
-
-Lemma inst_typing_eweak Σ Ξ d Γ ξ Ξ' :
-  inst_typing Σ Ξ Γ ξ Ξ' →
-  inst_typing Σ (d :: Ξ) Γ ξ Ξ'.
-Proof.
-  intros h.
-  eapply inst_typing_eweak_.
-  eapply inst_typing_impl; eauto.
-  apply typing_eweak.
-Qed.
-
-Lemma wf_eweak Σ Ξ d Γ :
-  wf Σ Ξ Γ →
-  wf Σ (d :: Ξ) Γ.
-Proof.
-  intros h. induction h.
-  - constructor.
-  - econstructor.
-    + assumption.
-    + eapply typing_eweak. eassumption.
-Qed.
-
-Lemma equation_typing_eweak Σ Ξ d r :
-  equation_typing Σ Ξ r →
-  equation_typing Σ (d :: Ξ) r.
-Proof.
-  intros (hctx & [i hty] & hl & hr).
-  unfold equation_typing.
-  intuition eauto using typing_eweak, wf_eweak.
-Qed.
-
-(** Global environment weakening *)
-
-Lemma inst_equations_gweak_ih Σ Σ' Ξ ξ Ξ' :
-  Σ ⊑ Σ' →
-  inst_equations_ (λ u v, Σ' ;; Ξ ⊢ u ≡ v) ξ Ξ' →
-  inst_equations Σ' Ξ ξ Ξ'.
-Proof.
-  intros hle ih.
-  intros x rl hx. specialize (ih _ _ hx).
-  intuition eauto.
-Qed.
-
-Lemma conv_gweak Σ Σ' Ξ u v :
-  Σ ;; Ξ ⊢ u ≡ v →
-  Σ ⊑ Σ' →
-  Σ' ;; Ξ ⊢ u ≡ v.
-Proof.
-  intros h hle. induction h using conversion_ind.
-  all: solve [ econstructor ; eauto ].
-Qed.
-
-Lemma inst_equations_gweak Σ Σ' Ξ ξ Ξ' :
-  inst_equations Σ Ξ ξ Ξ' →
-  Σ ⊑ Σ' →
-  inst_equations Σ' Ξ ξ Ξ'.
-Proof.
-  intros h hle.
-  eauto using inst_equations_gweak_ih, inst_equations_prop, conv_gweak.
-Qed.
-
-Lemma inst_iget_gweak Σ Σ' Ξ Γ ξ Ξ' :
-  inst_iget Σ Ξ Γ ξ Ξ' →
-  inst_iget_ (λ Γ t A, Σ' ;; Ξ | Γ ⊢ t : A) Γ ξ Ξ' →
-  Σ ⊑ Σ' →
-  inst_iget Σ' Ξ Γ ξ Ξ'.
-Proof.
-  intros h ih hle. auto.
-Qed.
-
-Lemma inst_typing_gweak_ Σ Σ' Ξ Γ ξ Ξ' :
-  inst_typing_ (conversion Σ Ξ) (λ t A, Σ' ;; Ξ | Γ ⊢ t : A) ξ Ξ' →
-  Σ ⊑ Σ' →
-  inst_typing Σ' Ξ Γ ξ Ξ'.
-Proof.
-  induction 1; constructor; eauto.
-  eapply conv_gweak; eauto.
-Qed.
-
-Lemma typing_gweak Σ Σ' Ξ Γ t A :
-  Σ ;; Ξ | Γ ⊢ t : A →
-  Σ ⊑ Σ' →
-  Σ' ;; Ξ | Γ ⊢ t : A.
-Proof.
-  intros h hle. induction h using typing_ind.
-  all: try solve [ econstructor ; eauto ].
-  - econstructor. 1,3: eauto.
-    eapply inst_typing_gweak_. all: eassumption.
-  - econstructor. 1,3: eassumption.
-    eapply conv_gweak. all: eauto.
-Qed.
-
-Lemma inst_typing_gweak Σ Σ' Ξ Γ ξ Ξ' :
-  inst_typing Σ Ξ Γ ξ Ξ' →
-  Σ ⊑ Σ' →
-  inst_typing Σ' Ξ Γ ξ Ξ'.
-Proof.
-  intros h hle.
-  eapply inst_typing_gweak_; eauto.
-  eapply inst_typing_impl; eauto.
-  intros; eapply typing_gweak; eauto.
-Qed.
-
-Lemma gscope_gweak Σ Σ' t :
-  gscope Σ t →
-  Σ ⊑ Σ' →
-  gscope Σ' t.
-Proof.
-  intros h hle.
-  induction h using gscope_ind.
-  all: solve [ econstructor ; eauto ].
-Qed.
-
-Lemma gscope_crule_gweak Σ Σ' rl :
-  gscope_crule Σ rl →
-  Σ ⊑ Σ' →
-  gscope_crule Σ' rl.
-Proof.
-  intros h hle.
-  destruct h. split.
-  all: intuition eauto using Forall_impl, gscope_gweak.
-Qed.
-
-Lemma wf_gweak Σ Σ' Ξ Γ :
-  wf Σ Ξ Γ →
-  Σ ⊑ Σ' →
-  wf Σ' Ξ Γ.
-Proof.
-  intros h hle. induction h.
-  - constructor.
-  - econstructor.
-    + assumption.
-    + eapply typing_gweak. all: eassumption.
-Qed.
-
-Lemma equation_typing_gweak Σ Σ' Ξ r :
-  equation_typing Σ Ξ r →
-  Σ ⊑ Σ' →
-  equation_typing Σ' Ξ r.
-Proof.
-  intros (hctx & [i hty] & hl & hr) hle.
-  unfold equation_typing.
-  intuition eauto using typing_gweak, wf_gweak.
-Qed.
-
-Lemma iwf_gweak Σ Σ' Ξ :
-  iwf Σ Ξ →
-  Σ ⊑ Σ' →
-  iwf Σ' Ξ.
-Proof.
-  intros h hle. induction h.
-  - constructor.
-  - econstructor. 1: assumption.
-    eapply typing_gweak. all: eassumption.
-  - econstructor.
-    + assumption.
-    + eapply gscope_crule_gweak. all: eassumption.
-    + assumption.
-    + eapply equation_typing_gweak. all: eassumption.
-Qed.
-
-Lemma wf_rules_gweak Σ Σ' Ξ R :
-  Forall (equation_typing Σ Ξ) R →
-  Σ ⊑ Σ' →
-  Forall (equation_typing Σ' Ξ) R.
-Proof.
-  intros h hle.
-  eapply Forall_impl. 2: eassumption.
-  intros. eauto using equation_typing_gweak.
-Qed.
-
 (** Validity (or presupposition) *)
 
-Lemma styping_ids Σ Ξ Γ :
-  styping Σ Ξ Γ ids Γ.
+Lemma σtyping_ids Γ :
+  σtyping Γ ids Γ.
 Proof.
   induction Γ as [| A Γ ih].
   - constructor.
   - constructor.
-    + eapply styping_weak with (A := A) in ih.
+    + eapply σtyping_weak with (A := A) in ih.
       assumption.
-    + eapply meta_conv.
-      * econstructor. cbn. reflexivity.
-      * rasimpl. substify. reflexivity.
+    + assert (Init.Nat.add 1 ⋅ A = A <[ S >> ids]) as <- by now rasimpl; substify.
+      now econstructor.
 Qed.
 
-Lemma styping_one Σ Ξ Γ A u :
-  Σ ;; Ξ | Γ ⊢ u : A →
-  styping Σ Ξ Γ u.. (Γ ,, A).
+Lemma styping_one Γ A u :
+  Γ ⊢ u : A →
+  σtyping Γ u.. (Γ ,, A).
 Proof.
   intros h.
   constructor. all: rasimpl. 2: auto.
-  erewrite autosubst_simpl_styping. 2: exact _. (* Somehow rasimpl doesn't work *)
-  apply styping_ids.
+  erewrite autosubst_simpl_σtyping. 2: exact _. (* Somehow rasimpl doesn't work *)
+  apply σtyping_ids.
 Qed.
 
-Lemma valid_wf Σ Ξ Γ x A :
-  wf Σ Ξ Γ →
+Lemma valid_wf Γ x A :
+  wf Γ →
   nth_error Γ x = Some A →
-  ∃ i, Σ ;; Ξ | Γ ⊢ (plus (S x)) ⋅ A : Sort i.
+  ∃ i, Γ ⊢ (plus (S x)) ⋅ A : Typ i ∨ Γ ⊢ (plus (S x)) ⋅ A : PTyp i.
 Proof.
   intros hΓ h.
   induction hΓ as [| Γ i B hΓ ih hB] in x, h |- *.
   1: destruct x ; discriminate.
   destruct x.
-  + cbn in *. inversion h. subst.
+  - cbn in *. inversion h. subst.
     exists i. rasimpl.
-    eapply meta_conv.
-    * eapply typing_ren. 1: eapply rtyping_S.
-      eassumption.
-    * reflexivity.
-  + cbn in h. eapply ih in h as [j h]. exists j.
-    eapply typing_ren in h. 2: eapply rtyping_S.
-    rasimpl in h. eassumption.
+    destruct hB as [hB1|hB2].
+    + left. assert (S ⋅ Typ i = Typ i) as <- by easy.
+      eapply styping_ren. 1: eapply rtyping_S.
+      assumption.
+    + right. assert (S ⋅ PTyp i = PTyp i) as <- by easy.
+      eapply styping_ren. 1: eapply rtyping_S.
+      assumption.
+  - cbn in h. eapply ih in h as [j h]. exists j.
+    destruct h as [h1|h2].
+    + left. eapply styping_ren in h1. 2: eapply rtyping_S.
+      rasimpl in h1. eassumption.
+    + right. eapply styping_ren in h2. 2: eapply rtyping_S.
+      rasimpl in h2. eassumption.
 Qed.
 
-Lemma ictx_get_case d Ξ M i :
-  ictx_get (d :: Ξ) M = Some i →
-  (M = length Ξ ∧ d = i) ∨ (ictx_get Ξ M = Some i).
-Proof.
-  intro h.
-  unfold ictx_get in h. rewrite nth_error_rev in h.
-  destruct (_ <? _) eqn: e. 2: discriminate.
-  rewrite Nat.ltb_lt in e. cbn in e.
-  cbn in h.
-  destruct (length Ξ - M) eqn: e'.
-  - left. cbn in h. inversion h.
-    intuition lia.
-  - right. cbn in h.
-    unfold ictx_get.
-    rewrite nth_error_rev.
-    destruct (_ <? _) eqn: e2.
-    2:{ rewrite Nat.ltb_ge in e2. lia. }
-    rewrite <- h. f_equal. lia.
-Qed.
-
-Lemma valid_assm Σ Ξ x A :
-  iwf Σ Ξ →
-  ictx_get Ξ x = Some (Assm A) →
-  ∃ i, Σ ;; Ξ | ∙ ⊢ A : Sort i.
-Proof.
-  intros hΞ e.
-  induction hΞ as [| B Ξ i hΞ ih hB | rl Ξ hΞ ih hs ht ].
-  - destruct x. all: discriminate.
-  - eapply ictx_get_case in e as eh. destruct eh as [[-> eh] | eh].
-    + inversion eh. subst.
-      eexists. eapply typing_eweak. eassumption.
-    + specialize (ih eh) as [].
-      eexists. eapply typing_eweak. eassumption.
-  - eapply ictx_get_case in e as eh. destruct eh as [[-> eh] | eh].
-    1: discriminate.
-    specialize (ih eh) as [].
-    eexists. eapply typing_eweak. eassumption.
-Qed.
-
-Lemma valid_comp Σ Ξ x rl :
-  iwf Σ Ξ →
-  ictx_get Ξ x = Some (Comp rl) →
-  gscope_crule Σ rl ∧ equation_typing Σ Ξ (crule_eq rl).
-Proof.
-  intros hΞ e.
-  induction hΞ as [| B Ξ i hΞ ih hB | rl' Ξ hΞ ih hs ht ].
-  - destruct x. all: discriminate.
-  - eapply ictx_get_case in e as eh. destruct eh as [[-> eh] | eh].
-    1: discriminate.
-    intuition eauto using equation_typing_eweak.
-  - eapply ictx_get_case in e as eh. destruct eh as [[-> eh] | eh].
-    + inversion eh. subst.
-      intuition eauto using equation_typing_eweak.
-    + specialize (ih eh) as [].
-      intuition eauto using equation_typing_eweak.
-Qed.
-
-Lemma extends_nil Σ :
-  [] ⊑ Σ.
-Proof.
-  intros ?? e. discriminate.
-Qed.
-
-Lemma extends_gcons (Σ : gctx) c d :
-  Σ c = None →
-  Σ ⊑ (c, d) :: Σ.
-Proof.
-  intros h. intros c' d' e.
-  cbn. destruct (_ =? _)%string eqn:ec.
-  - apply eqb_eq in ec. subst. congruence.
-  - assumption.
-Qed.
-
-Lemma valid_def Σ c Ξ A t :
-  gwf Σ →
-  Σ c = Some (Def Ξ A t) →
-  iwf Σ Ξ ∧
-  (∃ i, Σ ;; Ξ | ∙ ⊢ A : Sort i) ∧
-  Σ ;; Ξ | ∙ ⊢ t : A.
-Proof.
-  intros hΣ hc.
-  induction hΣ as [ | c' ??????? ih ] in c, Ξ, A, t, hc |- *.
-  - discriminate.
-  - cbn in hc. destruct (c =? c')%string.
-    + inversion hc. subst.
-      intuition eauto using iwf_gweak, typing_gweak, extends_gcons.
-    + specialize ih with (1 := hc) as [? [[j ?] ?]].
-      intuition eauto using iwf_gweak, typing_gweak, extends_gcons.
-Qed.
-
-Definition styping_alt Σ Ξ (Γ : ctx) (σ : nat → term) (Δ : ctx) :=
+Definition σtyping_alt (Γ : ctx) (σ : nat → term) (Δ : ctx) :=
   ∀ x A,
     nth_error Δ x = Some A →
-    Σ ;; Ξ | Γ ⊢ σ x : ((plus (S x)) ⋅ A) <[ σ ].
+    Γ ⊢ σ x : ((plus (S x)) ⋅ A) <[ σ ].
 
-Lemma styping_alt_equiv Σ Ξ Γ σ Δ :
-  styping Σ Ξ Γ σ Δ ↔ styping_alt Σ Ξ Γ σ Δ.
+Lemma σtyping_alt_equiv Γ σ Δ :
+  σtyping Γ σ Δ ↔ σtyping_alt Γ σ Δ.
 Proof.
   split.
   - intro h. induction h as [| ???? ih].
@@ -2251,128 +762,228 @@ Proof.
       assumption.
 Qed.
 
-Lemma typing_lift_closed Σ Ξ Γ t A :
-  Σ ;; Ξ | ∙ ⊢ t : A →
+Lemma styping_lift_closed Γ t A :
+  ∙ ⊢ t : A →
   closed A = true →
-  Σ ;; Ξ | Γ ⊢ t : A.
+  Γ ⊢ t : A.
 Proof.
   intros h hA.
-  eapply typing_scoped in h as ht. cbn in ht.
-  eapply typing_ren in h. 2: eapply rtyping_add.
+  eapply styping_scoped in h as ht. cbn in ht.
+  eapply styping_ren in h. 2: eapply rtyping_add.
   rewrite !closed_ren in h. 2,3: assumption.
   rewrite app_nil_r in h.
   eassumption.
 Qed.
 
-Lemma validity Σ Ξ Γ t A :
-  gwf Σ →
-  iwf Σ Ξ →
-  wf Σ Ξ Γ →
-  Σ ;; Ξ | Γ ⊢ t : A →
-  ∃ i, Σ ;; Ξ | Γ ⊢ A : Sort i.
+Lemma validity Γ t A :
+  wf Γ →
+  Γ ⊢ t : A →
+  ∃ i, Γ ⊢ A : Typ i ∨ Γ ⊢ A : PTyp i.
 Proof.
-  intros hΣ hΞ hΓ h.
-  induction h using typing_ind in hΓ |- *.
+  intros hΓ h.
+  induction h using styping_ind in hΓ |- *.
   all: try solve [ eexists ; econstructor ; eauto ].
   - apply valid_wf. all: assumption.
-  - eexists. eapply meta_conv.
-    + eapply typing_subst.
-      * eapply styping_one. eassumption.
-      * eassumption.
-    + reflexivity.
-  - eapply valid_def in hΣ as h. 2: eassumption.
-    destruct h as [? [[i ?]]].
-    exists i. eapply meta_conv.
-    + eapply typing_inst_closed. all: eassumption.
-    + reflexivity.
-  - eapply valid_assm in hΞ as h. 2: eassumption.
-    destruct h as [i hA].
-    exists i. eapply typing_lift_closed. 2: reflexivity.
-    assumption.
-  - eexists. eassumption.
+  - exists (S (S i)). left; constructor.
+  - exists (S (S i)). right; constructor.
+  - exists (S (Nat.max i j)). left; constructor.
+  - exists (S (Nat.max i j)). right; constructor.
+  - exists (S (Nat.max i j)). left; constructor.
+  - exists (S (Nat.max i j)). right; constructor.
+  - exists (Nat.max i j). left; constructor; auto.
+  - exists (Nat.max i j). right; constructor; auto.
+  - exists (Nat.max i j). left; constructor; auto.
+  - exists (Nat.max i j). right; constructor; auto.
+  - exists j; left.
+    assert (Typ j <[ u..] = Typ j) as <- by easy.
+    apply (styping_subst (Γ,,A)).
+    + now apply styping_one.
+    + assumption.
+  - exists j; right.
+    assert (PTyp j <[ u..] = PTyp j) as <- by easy.
+    apply (styping_subst (Γ,,A)).
+    + now apply styping_one.
+    + assumption.
+  - exists j; left.
+    assert (Typ j <[ u..] = Typ j) as <- by easy.
+    apply (styping_subst (Γ,,A)).
+    + now apply styping_one.
+    + assumption.
+  - exists j; right.
+    assert (PTyp j <[ u..] = PTyp j) as <- by easy.
+    apply (styping_subst (Γ,,A)).
+    + now apply styping_one.
+    + assumption.
 Qed.
 
 (** Induction principle for [typing], threading [wf] *)
 
 Lemma typing_ind_wf :
-  ∀ Σ Ξ (P : ctx → term → term → Prop),
+  ∀ (P : ctx → term → term → Prop),
     (∀ Γ x A,
-      wf Σ Ξ Γ →
+      wf Γ →
       nth_error Γ x = Some A →
       P Γ (var x) (Nat.add (S x) ⋅ A)
     ) →
-    (∀ Γ i, wf Σ Ξ Γ → P Γ (Sort i) (Sort (S i))) →
+    (∀ Γ i, wf Γ → P Γ (Typ i) (Typ (S i))) →
+    (∀ Γ i, wf Γ → P Γ (PTyp i) (PTyp (S i))) →
+    
     (∀ Γ i j A B,
-      wf Σ Ξ Γ →
-      Σ ;; Ξ | Γ ⊢ A : Sort i →
-      P Γ A (Sort i) →
-      Σ ;; Ξ | Γ,, A ⊢ B : Sort j →
-      P (Γ,, A) B (Sort j) →
-      P Γ (Pi A B) (Sort (Nat.max i j))
+      wf Γ →
+      Γ ⊢ A : Typ i →
+      P Γ A (Typ i) →
+      Γ,, A ⊢ B : Typ j →
+      P (Γ,, A) B (Typ j) →
+      P Γ (Pi A B) (Typ (Nat.max i j))
     ) →
+    (∀ Γ i j A B,
+      wf Γ →
+      Γ ⊢ A : PTyp i →
+      P Γ A (PTyp i) →
+      Γ,, A ⊢ B : PTyp j →
+      P (Γ,, A) B (PTyp j) →
+      P Γ (Pi A B) (PTyp (Nat.max i j))
+    ) →
+    (∀ Γ i j A B,
+      wf Γ →
+      Γ ⊢ A : PTyp i →
+      P Γ A (PTyp i) →
+      Γ,, A ⊢ B : Typ j →
+      P (Γ,, A) B (Typ j) →
+      P Γ (Pi A B) (Typ (Nat.max i j))
+    ) →
+    (∀ Γ i j A B,
+      wf Γ →
+      Γ ⊢ A : Typ i →
+      P Γ A (Typ i) →
+      Γ,, A ⊢ B : PTyp j →
+      P (Γ,, A) B (PTyp j) →
+      P Γ (Pi A B) (PTyp (Nat.max i j))
+    ) →
+    
     (∀ Γ i j A B t,
-      wf Σ Ξ Γ →
-      Σ ;; Ξ | Γ ⊢ A : Sort i →
-      P Γ A (Sort i) →
-      Σ ;; Ξ | Γ,, A ⊢ B : Sort j →
-      P (Γ,, A) B (Sort j) →
-      Σ ;; Ξ | Γ,, A ⊢ t : B →
+      wf Γ →
+      Γ ⊢ A : Typ i →
+      P Γ A (Typ i) →
+      Γ,, A ⊢ B : Typ j →
+      P (Γ,, A) B (Typ j) →
+      Γ,, A ⊢ t : B →
       P (Γ,, A) t B → P Γ (lam A t) (Pi A B)
     ) →
+    (∀ Γ i j A B t,
+      wf Γ →
+      Γ ⊢ A : PTyp i →
+      P Γ A (PTyp i) →
+      Γ,, A ⊢ B : PTyp j →
+      P (Γ,, A) B (PTyp j) →
+      Γ,, A ⊢ t : B →
+      P (Γ,, A) t B → P Γ (lam A t) (Pi A B)
+    ) →(∀ Γ i j A B t,
+      wf Γ →
+      Γ ⊢ A : PTyp i →
+      P Γ A (PTyp i) →
+      Γ,, A ⊢ B : Typ j →
+      P (Γ,, A) B (Typ j) →
+      Γ,, A ⊢ t : B →
+      P (Γ,, A) t B → P Γ (lam A t) (Pi A B)
+    ) →(∀ Γ i j A B t,
+      wf Γ →
+      Γ ⊢ A : Typ i →
+      P Γ A (Typ i) →
+      Γ,, A ⊢ B : PTyp j →
+      P (Γ,, A) B (PTyp j) →
+      Γ,, A ⊢ t : B →
+      P (Γ,, A) t B → P Γ (lam A t) (Pi A B)
+    ) →
+    
     (∀ Γ i j A B t u,
-      wf Σ Ξ Γ →
-      Σ ;; Ξ | Γ ⊢ t : Pi A B →
+      wf Γ →
+      Γ ⊢ t : Pi A B →
       P Γ t (Pi A B) →
-      Σ ;; Ξ | Γ ⊢ u : A →
-      P Γ u A → Σ ;; Ξ | Γ ⊢ A : Sort i →
-      P Γ A (Sort i) → Σ ;; Ξ | Γ,, A ⊢ B : Sort j →
-      P (Γ,, A) B (Sort j) →
+      Γ ⊢ u : A →
+      P Γ u A → Γ ⊢ A : Typ i →
+      P Γ A (Typ i) → Γ,, A ⊢ B : Typ j →
+      P (Γ,, A) B (Typ j) →
       P Γ (app t u) (B <[ u..])
     ) →
-    (∀ Γ c ξ Ξ' A t,
-      wf Σ Ξ Γ →
-      Σ c = Some (Def Ξ' A t) →
-      inst_typing Σ Ξ Γ ξ Ξ' →
-      inst_typing_ (conversion Σ Ξ) (λ t A, wf Σ Ξ Γ → P Γ t A) ξ Ξ' →
-      closed A = true →
-      P Γ (const c ξ) (inst ξ A)
+    (∀ Γ i j A B t u,
+      wf Γ →
+      Γ ⊢ t : Pi A B →
+      P Γ t (Pi A B) →
+      Γ ⊢ u : A →
+      P Γ u A → Γ ⊢ A : PTyp i →
+      P Γ A (PTyp i) → Γ,, A ⊢ B : PTyp j →
+      P (Γ,, A) B (PTyp j) →
+      P Γ (app t u) (B <[ u..])
     ) →
-    (∀ Γ x A,
-      wf Σ Ξ Γ →
-      ictx_get Ξ x = Some (Assm A) →
-      closed A = true →
-      P Γ (assm x) A
+    (∀ Γ i j A B t u,
+      wf Γ →
+      Γ ⊢ t : Pi A B →
+      P Γ t (Pi A B) →
+      Γ ⊢ u : A →
+      P Γ u A → Γ ⊢ A : PTyp i →
+      P Γ A (PTyp i) → Γ,, A ⊢ B : Typ j →
+      P (Γ,, A) B (Typ j) →
+      P Γ (app t u) (B <[ u..])
     ) →
+    (∀ Γ i j A B t u,
+      wf Γ →
+      Γ ⊢ t : Pi A B →
+      P Γ t (Pi A B) →
+      Γ ⊢ u : A →
+      P Γ u A → Γ ⊢ A : Typ i →
+      P Γ A (Typ i) → Γ,, A ⊢ B : PTyp j →
+      P (Γ,, A) B (PTyp j) →
+      P Γ (app t u) (B <[ u..])
+    ) →
+    
     (∀ Γ i A B t,
-      wf Σ Ξ Γ →
-      Σ ;; Ξ | Γ ⊢ t : A →
+      wf Γ →
+      Γ ⊢ t : A →
       P Γ t A →
-      Σ ;; Ξ ⊢ A ≡ B →
-      Σ ;; Ξ | Γ ⊢ B : Sort i →
-      P Γ B (Sort i) →
+      A ≡ B →
+      Γ ⊢ B : Typ i →
+      P Γ B (Typ i) →
       P Γ t B
     ) →
-    ∀ Γ t A, wf Σ Ξ Γ → Σ ;; Ξ | Γ ⊢ t : A → P Γ t A.
+    (∀ Γ i A B t,
+      wf Γ →
+      Γ ⊢ t : A →
+      P Γ t A →
+      A ≡ B →
+      Γ ⊢ B : PTyp i →
+      P Γ B (PTyp i) →
+      P Γ t B
+    ) →
+    
+    ∀ Γ t A, wf Γ → Γ ⊢ t : A → P Γ t A.
 Proof.
-  intros Σ Ξ P hvar hsort hpi hlam happ hconst hassm hconv.
+  intros P hvar htyp hptyp hpiT hpiP hpiPT hpiTP
+    hlamT hlamP hlamPT hlamTP happT happP happPT happTP hconvT hconvP.
   intros Γ t A hΓ h.
-  induction h using typing_ind.
+  induction h using styping_ind.
   all: try solve [ eauto using wf_cons ].
-  - assert (hΓA : wf Σ Ξ (Γ ,, A)).
-    { econstructor. all: eassumption. }
-    eauto.
-  - assert (hΓA : wf Σ Ξ (Γ ,, A)).
-    { econstructor. all: eassumption. }
-    eapply happ. all: eauto.
+  - apply hpiT; eauto using wf_cons.
+  - apply hpiP; eauto using wf_cons.
+  - apply hpiPT; eauto using wf_cons.
+  - apply hpiTP; eauto using wf_cons.
+  - apply (hlamT _ i j); eauto using wf_cons.
+  - apply (hlamP _ i j); eauto using wf_cons.
+  - apply (hlamPT _ i j); eauto using wf_cons.
+  - apply (hlamTP _ i j); eauto using wf_cons.
+  - apply (happT _ i j A); eauto using wf_cons.
+  - apply (happP _ i j A); eauto using wf_cons.
+  - apply (happPT _ i j A); eauto using wf_cons.
+  - apply (happTP _ i j A); eauto using wf_cons.
 Qed.
 
 (** * Context conversion *)
 
-Notation ctx_conv Σ Ξ Γ Δ := (Forall2 (conversion Σ Ξ) Γ Δ).
+Notation ctx_conv Γ Δ := (Forall2 conversion Γ Δ).
 
-Lemma ctx_conv_cons_same Σ Ξ Γ Δ A :
-  ctx_conv Σ Ξ Γ Δ →
-  ctx_conv Σ Ξ (Γ ,, A) (Δ ,, A).
+Lemma ctx_conv_cons_same Γ Δ A :
+  ctx_conv Γ Δ →
+  ctx_conv (Γ ,, A) (Δ ,, A).
 Proof.
   intros h.
   constructor.
@@ -2380,16 +991,16 @@ Proof.
   - assumption.
 Qed.
 
-Lemma ctx_conv_refl Σ Ξ Γ :
-  ctx_conv Σ Ξ Γ Γ.
+Lemma ctx_conv_refl Γ :
+  ctx_conv Γ Γ.
 Proof.
   apply Forall2_diag. apply Forall_forall.
   auto using conv_refl.
 Qed.
 
-Lemma ctx_conv_cons_same_ctx Σ Ξ Γ A B :
-  Σ ;; Ξ ⊢ A ≡ B →
-  ctx_conv Σ Ξ (Γ ,, A) (Γ ,, B).
+Lemma ctx_conv_cons_same_ctx Γ A B :
+  A ≡ B →
+  ctx_conv (Γ ,, A) (Γ ,, B).
 Proof.
   intros h.
   constructor.
@@ -2397,70 +1008,112 @@ Proof.
   - apply ctx_conv_refl.
 Qed.
 
-Inductive wf_ctx_conv Σ Ξ : ctx → ctx → Prop :=
-| wf_conv_nil : wf_ctx_conv Σ Ξ ∙ ∙
+Inductive wf_ctx_conv : ctx → ctx → Prop :=
+| wf_conv_nil : wf_ctx_conv ∙ ∙
 | wf_conv_cons Γ Δ i A B :
-    wf_ctx_conv Σ Ξ Γ Δ →
-    Σ ;; Ξ | Δ ⊢ A : Sort i →
-    Σ ;; Ξ ⊢ A ≡ B →
-    wf_ctx_conv Σ Ξ (Γ ,, A) (Δ ,, B).
+    wf_ctx_conv Γ Δ →
+    Δ ⊢ A : Typ i ∨ Δ ⊢ A : PTyp i →
+    A ≡ B →
+    wf_ctx_conv (Γ ,, A) (Δ ,, B).
 
-Lemma wf_ctx_conv_nth_error_l Σ Ξ Γ Δ x A :
-  wf_ctx_conv Σ Ξ Γ Δ →
+Lemma wf_ctx_conv_nth_error_l Γ Δ x A :
+  wf_ctx_conv Γ Δ →
   nth_error Γ x = Some A →
   ∃ i B,
     nth_error Δ x = Some B ∧
-    Σ ;; Ξ ⊢ A ≡ B ∧
-    Σ ;; Ξ | Δ ⊢ (plus (S x)) ⋅ A : Sort i.
+    A ≡ B ∧
+    (Δ ⊢ (plus (S x)) ⋅ A : Typ i ∨ Δ ⊢ (plus (S x)) ⋅ A : PTyp i).
 Proof.
   intros hctx h.
-  induction hctx as [| Γ Δ i B C hctx ih hB he] in x, h |- *.
+  induction hctx as [| Γ Δ i B C hctx ih [hB1|hB2] he] in x, h |- *.
   1: destruct x ; discriminate.
-  destruct x.
-  - cbn in *. inversion h. subst.
-    exists i, C. rasimpl. intuition auto.
-    eapply meta_conv.
-    + eapply typing_ren. 1: eapply rtyping_S.
+  - destruct x.
+    + simpl in *. inversion h. subst.
+      exists i, C. rasimpl. intuition auto. left.
+      assert (S ⋅ Typ i = Typ i) as <- by easy.
+      eapply styping_ren. 1: eapply rtyping_S.
       eassumption.
-    + reflexivity.
-  - cbn in h. eapply ih in h as (j & D & ? & ? & h).
-    exists j, D. cbn. intuition auto.
-    eapply typing_ren in h. 2: eapply rtyping_S.
-    rasimpl in h. eassumption.
+    + cbn in h. eapply ih in h as (j & D & ? & ? & h).
+      destruct h as [h1|h2].
+      * exists j, D. cbn. intuition auto. left.
+        eapply styping_ren in h1. 2: eapply rtyping_S.
+        rasimpl in h1. eassumption.
+      * exists j, D. cbn. intuition auto. right.
+        eapply styping_ren in h2. 2: eapply rtyping_S.
+        rasimpl in h2. eassumption.
+  - destruct x.
+    + simpl in *. inversion h. subst.
+      exists i, C. rasimpl. intuition auto. right.
+      assert (S ⋅ PTyp i = PTyp i) as <- by easy.
+      eapply styping_ren. 1: eapply rtyping_S.
+      eassumption.
+    + cbn in h. eapply ih in h as (j & D & ? & ? & h).
+      destruct h as [h1|h2].
+      * exists j, D. cbn. intuition auto. left.
+        eapply styping_ren in h1. 2: eapply rtyping_S.
+        rasimpl in h1. eassumption.
+      * exists j, D. cbn. intuition auto. right.
+        eapply styping_ren in h2. 2: eapply rtyping_S.
+        rasimpl in h2. eassumption.
 Qed.
 
-Lemma inst_typing_ctx_conv_ih Σ Ξ Ξ' (Γ Δ : ctx) ξ :
-  wf_ctx_conv Σ Ξ Γ Δ →
-  inst_typing_ (conversion Σ Ξ) (λ t A, ∀ Δ, wf_ctx_conv Σ Ξ Γ Δ → Σ ;; Ξ | Δ ⊢ t : A) ξ Ξ' →
-  inst_typing Σ Ξ Δ ξ Ξ'.
-Proof.
-  intros hctx.
-  induction 1; constructor; eauto.
-Qed.
-
-Lemma typing_ctx_conv_gen Σ Ξ (Γ Δ : ctx) t A :
-  wf_ctx_conv Σ Ξ Γ Δ →
-  Σ ;; Ξ | Γ ⊢ t : A →
-  Σ ;; Ξ | Δ ⊢ t : A.
+Lemma typing_ctx_conv_gen (Γ Δ : ctx) t A :
+  wf_ctx_conv Γ Δ →
+  Γ ⊢ t : A →
+  Δ ⊢ t : A.
 Proof.
   intros hctx h.
-  induction h in Δ, hctx |- * using typing_ind.
+  induction h in Δ, hctx |- * using styping_ind.
   all: try solve [ econstructor ; eauto using wf_conv_cons, conv_refl ].
   - eapply wf_ctx_conv_nth_error_l in hctx as h. 2: eassumption.
     destruct h as (i & B & e & hc & h).
-    eapply type_conv.
+    eapply stype_conv.
     + econstructor. eassumption.
     + apply conv_sym. apply conv_ren. assumption.
     + eassumption.
-  - econstructor. 1,3: eassumption.
-    eauto using inst_typing_ctx_conv_ih.
+  - econstructor.
+    + left. now eapply IHh1.
+    + left. eapply IHh2.
+      apply (wf_conv_cons _ _ i); auto using conv_refl.
+    + apply IHh3.
+      apply (wf_conv_cons _ _ i); auto using conv_refl.
+  - econstructor.
+    + right. now eapply IHh1.
+    + right. eapply IHh2.
+      apply (wf_conv_cons _ _ i); auto using conv_refl.
+    + apply IHh3.
+      apply (wf_conv_cons _ _ i); auto using conv_refl.
+  - econstructor.
+    + right. now eapply IHh1.
+    + left. eapply IHh2.
+      apply (wf_conv_cons _ _ i); auto using conv_refl.
+    + apply IHh3.
+      apply (wf_conv_cons _ _ i); auto using conv_refl.
+  - econstructor.
+    + left. now eapply IHh1.
+    + right. eapply IHh2.
+      apply (wf_conv_cons _ _ i); auto using conv_refl.
+    + apply IHh3.
+      apply (wf_conv_cons _ _ i); auto using conv_refl.
+  - econstructor; auto.
+    left. apply IHh4.
+    apply (wf_conv_cons _ _ i); auto using conv_refl.
+  - econstructor; auto.
+    right. apply IHh4.
+    apply (wf_conv_cons _ _ i); auto using conv_refl.
+  - econstructor; auto.
+    left. apply IHh4.
+    apply (wf_conv_cons _ _ i); auto using conv_refl.
+  - econstructor; auto.
+    right. apply IHh4.
+    apply (wf_conv_cons _ _ i); auto using conv_refl.
 Qed.
 
-Lemma typing_ctx_conv Σ Ξ (Γ Δ : ctx) t A :
-  Σ ;; Ξ | Γ ⊢ t : A →
-  wf Σ Ξ Γ →
-  ctx_conv Σ Ξ Γ Δ →
-  Σ ;; Ξ | Δ ⊢ t : A.
+Lemma typing_ctx_conv (Γ Δ : ctx) t A :
+  Γ ⊢ t : A →
+  wf Γ →
+  ctx_conv Γ Δ →
+  Δ ⊢ t : A.
 Proof.
   intros ht hΓ hctx.
   eapply typing_ctx_conv_gen. 2: eassumption.
@@ -2468,14 +1121,16 @@ Proof.
   - inversion hctx. constructor.
   - inversion hctx. subst.
     econstructor. 1,3: eauto.
-    eauto using typing_ctx_conv_gen.
+    destruct H.
+    + left; eauto using typing_ctx_conv_gen.
+    + right; eauto using typing_ctx_conv_gen.
 Qed.
 
 (** Congruence of substitution *)
 
-Lemma conv_substs_up Σ Ξ σ σ' :
-  (∀ x, Σ ;; Ξ ⊢ σ x ≡ σ' x) →
-  (∀ x, Σ ;; Ξ ⊢ up_term σ x ≡ up_term σ' x).
+Lemma conv_substs_up σ σ' :
+  (∀ x, σ x ≡ σ' x) →
+  (∀ x, up_term σ x ≡ up_term σ' x).
 Proof.
   intros h x.
   destruct x.
@@ -2483,20 +1138,12 @@ Proof.
   - cbn. unfold core.funcomp. apply conv_ren. auto.
 Qed.
 
-Lemma conv_substs Σ Ξ σ σ' t :
-  (∀ x, Σ ;; Ξ ⊢ σ x ≡ σ' x) →
-  Σ ;; Ξ ⊢ t <[ σ ] ≡ t <[ σ' ].
+Lemma conv_substs σ σ' t :
+  (∀ x, σ x ≡ σ' x) →
+  t <[ σ ] ≡ t <[ σ' ].
 Proof.
   intros h.
   induction t using term_rect in σ, σ', h |- *.
   all: try solve [ rasimpl ; econstructor ; eauto using conv_substs_up ].
-  - cbn. auto.
-  - cbn. econstructor.
-    apply Forall2_map_l, Forall2_map_r. apply Forall2_diag.
-    apply All_Forall. eapply All_impl. 2: eassumption.
-    intros o ho.
-    apply option_rel_map_l, option_rel_map_r.
-    apply option_rel_diag. apply OnSome_onSome. apply onSomeT_onSome.
-    eapply onSomeT_impl. 2: eassumption.
-    cbn. auto.
+  eauto.
 Qed.
