theories/BasicAST.v
@@ -2,11 +2,5 @@ From Stdlib Require Import Utf8 String.
 
 Set Primitive Projections.
 
-(** Reference in the global environment *)
-Definition gref := string.
-
-(** Reference to an assumption (de Bruijn level) *)
-Definition aref := nat.
-
 (** Universe level *)
 Definition level := nat.
