theories/Inst.v
@@ -9,45 +9,6 @@ Set Default Goal Selector "!".
 
 Open Scope subst_scope.
 
-Definition dummy := (Sort 0).
-
-Definition iget (ξ : instance) x :=
-  match nth_error ξ x with
-  | Some (Some t) => t
-  | _ => dummy
-  end.
-
-Notation map_instance f ξ :=
-  (map (option_map f) ξ).
-
-Notation ren_instance ρ ξ :=
-  (map_instance (ren_term ρ) ξ).
-
-Notation lift_instance ξ := (ren_instance S ξ).
-
-Notation liftn n ξ := (ren_instance (plus n) ξ).
-
-Fixpoint inst (ξ : instance) (t : term) :=
-  match t with
-  | var n => var n
-  | Sort i => Sort i
-  | Pi A B => Pi (inst ξ A) (inst (lift_instance ξ) B)
-  | lam A t => lam (inst ξ A) (inst (lift_instance ξ) t)
-  | app u v => app (inst ξ u) (inst ξ v)
-  | const c ξ' => const c (map_instance (inst ξ) ξ')
-  | assm x => iget ξ x
-  end.
-
-Notation inst_instance ξ ξ' := (map_instance (inst ξ) ξ').
-
-(** Instance for a context *)
-
-Fixpoint ctx_inst (ξ : instance) (Γ : ctx) : ctx :=
-  match Γ with
-  | [] => []
-  | A :: Γ => ctx_inst ξ Γ ,, inst (liftn (length Γ) ξ) A
-  end.
-
 (** ** Unrelated utility
 
   TODO MOVE
